tuned

TaskinBA/Complement/DPDA_Complement_HU.thy
@@ -1,6 +1,6 @@
-section \<open>Closure Property of DCFLs under Complementation\<close>
+section \<open>DCFLs are Closed Under Complementation\<close>
 
-theory Complement_DPDA
+theory DPDA_Complement_HU
   imports Det_Pushdown_Automata
 begin
 
@@ -8,36 +8,32 @@ subsection \<open>Setup and Auxiliary Lemmas\<close>
 
 context pda begin
 
-definition stepst :: "'q \<times> 'a list \<times> 's list \<Rightarrow> 'q \<times> 'a list \<times> 's list \<Rightarrow> bool"
-  ("(_ \<leadsto>+ _)" [50, 50] 50) where
-  "stepst \<equiv> step\<^sub>1 ^++"
+definition steps1 :: "'q \<times> 'a list \<times> 's list \<Rightarrow> 'q \<times> 'a list \<times> 's list \<Rightarrow> bool" (infix "\<leadsto>+" 55) where
+  "steps1 \<equiv> step\<^sub>1 ^++"
 
-abbreviation nstep\<^sub>1 ("(_ \<leadsto>)" [50] 50) where
-  "cf \<leadsto> \<equiv> (\<forall>cf'. \<not>cf \<leadsto> cf')"
+abbreviation no_step\<^sub>1 ("(_ \<leadsto>|)" [1000] 999) where
+  "cf \<leadsto>| \<equiv> (\<forall>cf'. \<not>cf \<leadsto> cf')"
 
-abbreviation nstepsn ("(_ /\<leadsto>'(_'))" [50, 0] 50) where
-  "cf \<leadsto>(n) \<equiv> (\<forall>cf'. \<not>cf \<leadsto>(n) cf')"
-
-lemma stepst_induct2[consumes 1]:
+lemma steps1_induct[consumes 1, case_names base step]:
   assumes "x1 \<leadsto>+ x2"
       and "\<And>q w \<alpha> p u \<gamma>. (q, w, \<alpha>) \<leadsto> (p, u, \<gamma>) \<Longrightarrow> P (q, w, \<alpha>) (p, u, \<gamma>)"
       and "\<And>q w \<alpha> r v \<beta> p u \<gamma>. (q, w, \<alpha>) \<leadsto> (r, v, \<beta>) \<Longrightarrow> (r, v, \<beta>) \<leadsto>+ (p, u, \<gamma>) \<Longrightarrow> 
                 P (r, v, \<beta>) (p, u, \<gamma>) \<Longrightarrow> P (q, w, \<alpha>) (p, u, \<gamma>)"
     shows "P x1 x2"
-using assms[unfolded stepst_def]
+using assms[unfolded steps1_def]
 proof(induction rule: converse_tranclp_induct)
   case base thus ?case by (metis prod_cases3)
 next
   case step thus ?case by simp (metis prod_cases3 step\<^sub>1.simps)
 qed
 
-lemma stepst_induct2_bw[consumes 1, case_names base step]:
+lemma steps1_converse_induct[consumes 1, case_names base step]:
   assumes "x1 \<leadsto>+ x2"
       and "\<And>q w \<alpha> p u \<gamma>. (q, w, \<alpha>) \<leadsto> (p, u, \<gamma>) \<Longrightarrow> P (q, w, \<alpha>) (p, u, \<gamma>)"
       and "\<And>q w \<alpha> r v \<beta> p u \<gamma>. (q, w, \<alpha>) \<leadsto>+ (r, v, \<beta>) \<Longrightarrow> (r, v, \<beta>) \<leadsto> (p, u, \<gamma>) \<Longrightarrow> 
                 P (q, w, \<alpha>) (r, v, \<beta>) \<Longrightarrow> P (q, w, \<alpha>) (p, u, \<gamma>)"
     shows "P x1 x2"
-  using assms[unfolded stepst_def]
+  using assms[unfolded steps1_def]
 proof(induction rule: tranclp_induct)
   case base
   then show ?case by (metis prod_cases3)
@@ -46,36 +42,28 @@ next
   then show ?case by simp (metis prod_cases3 step\<^sub>1.simps)
 qed
 
-lemma stepst_steps:
+lemma steps1_steps:
   "(q, w, \<alpha>) \<leadsto>+ (p, u, \<gamma>) \<Longrightarrow> (q, w, \<alpha>) \<leadsto>* (p, u, \<gamma>)"
-  by (simp add: steps_def stepst_def)
+  by (simp add: steps_def steps1_def)
 
-lemma stepst_step:
+lemma steps1_step:
   "(q, w, \<alpha>) \<leadsto> (p, u, \<gamma>) \<Longrightarrow> (q, w, \<alpha>) \<leadsto>+ (p, u, \<gamma>)"
-  by (simp add: stepst_def tranclp.r_into_trancl)
+  by (simp add: steps1_def tranclp.r_into_trancl)
 
-lemma stepst_trans:
+lemma steps1_trans:
   "(q, w, \<alpha>) \<leadsto>+ (p, u, \<gamma>) \<Longrightarrow> (p, u, \<gamma>) \<leadsto>+ (r, v, \<beta>) \<Longrightarrow> (q, w, \<alpha>) \<leadsto>+ (r, v, \<beta>)"
-using stepst_def by force
+using steps1_def by force
 
-lemma steps_stepst:
+lemma steps_steps1:
   assumes "(q, w, \<alpha>) \<leadsto>* (p, u, \<gamma>)"
       and "(q, w, \<alpha>) \<noteq> (p, u, \<gamma>)"
     shows "(q, w, \<alpha>) \<leadsto>+ (p, u, \<gamma>)"
-using assms unfolding steps_def stepst_def by (meson rtranclpD)
+using assms unfolding steps_def steps1_def by (meson rtranclpD)
 
-lemma stepst_split_last: "(\<exists>r v \<beta>. (q, w, \<alpha>) \<leadsto>* (r, v, \<beta>) \<and> (r, v, \<beta>) \<leadsto> (p, u, \<gamma>)) 
+lemma steps1_split_last: "(\<exists>r v \<beta>. (q, w, \<alpha>) \<leadsto>* (r, v, \<beta>) \<and> (r, v, \<beta>) \<leadsto> (p, u, \<gamma>)) 
                                 \<longleftrightarrow> (q, w, \<alpha>) \<leadsto>+ (p, u, \<gamma>)"
-proof
-  assume "\<exists>r v \<beta>. (q, w, \<alpha>) \<leadsto>* (r, v, \<beta>) \<and> (r, v, \<beta>) \<leadsto> (p, u, \<gamma>)"
-  then obtain r v \<beta> where "(q, w, \<alpha>) \<leadsto>* (r, v, \<beta>)" and "(r, v, \<beta>) \<leadsto> (p, u, \<gamma>)" by blast
-  then show "(q, w, \<alpha>) \<leadsto>+ (p, u, \<gamma>)"
-    by (simp add: steps_def stepst_def rtranclp_into_tranclp1)
-next
-  assume "(q, w, \<alpha>) \<leadsto>+ (p, u, \<gamma>)"
-  then show "\<exists>r v \<beta>. (q, w, \<alpha>) \<leadsto>* (r, v, \<beta>) \<and> (r, v, \<beta>) \<leadsto> (p, u, \<gamma>)"
-    by (induction rule: stepst_induct2_bw) (use steps_refl stepst_steps in blast)+
-qed
+by (smt (verit, ccfv_threshold) rtranclp_into_tranclp1 step\<^sub>1.elims(2) steps1_def steps_def steps_refl tranclp.simps
+      tranclp_into_rtranclp)
 
 lemma split_path:
   assumes "(q, w, \<alpha>) \<leadsto>(n) (p, [], \<gamma>)"
@@ -106,7 +94,7 @@ context dpda begin
 
 lemma max_eps_steps:
   assumes "(q, w, \<alpha>) \<leadsto>(n) (p, u, \<gamma>)"
-      and "(p, [], \<gamma>) \<leadsto>"
+      and "(p, [], \<gamma>) \<leadsto>|"
       and "(q, w, \<alpha>) \<leadsto>(m) (r, u, \<beta>)"
     shows "m \<le> n"
 proof (rule ccontr)
@@ -130,9 +118,10 @@ end
 text \<open>In what follows, we show that the complement of a deterministic context-free language is also a 
       deterministic context-free language. For this purpose, we construct a deterministic pushdown automaton 
       that recognizes the complement language of a given deterministic pushdown automaton. The proof 
-      follows that of Hopcroft and Ullman\cite{hopcroftullman}. The construction is divided into two parts: First, construct an equivalent 
+      follows that of Hopcroft and Ullman \cite{HopcroftU79}. The construction is divided into two parts: First, construct an equivalent 
       deterministic pushdown automaton that scans the entire input for all given input words, and then construct the automaton that recognizes the complement 
       language out of this automaton.\<close>
+
 
 subsection \<open>Scan Construction\<close>
 
@@ -142,40 +131,41 @@ text \<open>To scan the entire input, we address two complications: ensuring tha
       problem, we introduce a new final state that the automaton moves to if an infinite number of epsilon steps pass through 
       a final state; otherwise, the automaton moves to the dead state.\<close>
 
+
 subsubsection \<open>Definition\<close>
 
-datatype 'q st_extended = OST 'q | Q0' | D | F
-datatype 's sym_extended = OSYM 's | X0
+datatype 'q st_scan = St 'q | Q0' | D | F
+datatype 's sym_scan = Sym 's | X0
 
-lemma inj_OSYM: "inj OSYM"
+lemma inj_Sym: "inj Sym"
   by (simp add: inj_def)
 
-instance st_extended :: (finite) finite
+instance st_scan :: (finite) finite
 proof
-  have *: "UNIV = {t. \<exists>q. t = OST q} \<union> {Q0', D, F}"
-    by auto (metis st_extended.exhaust)
-  show "finite (UNIV :: 'a st_extended set)"
+  have *: "UNIV = {t. \<exists>q. t = St q} \<union> {Q0', D, F}"
+    by auto (metis st_scan.exhaust)
+  show "finite (UNIV :: 'a st_scan set)"
     by (simp add: * full_SetCompr_eq)
 qed
 
-instance sym_extended :: (finite) finite
+instance sym_scan :: (finite) finite
 proof
-  have *: "UNIV = {t. \<exists>q. t = OSYM q} \<union> {X0}"
-    by auto (metis sym_extended.exhaust)
-  show "finite (UNIV :: 'a sym_extended set)"
+  have *: "UNIV = {t. \<exists>q. t = Sym q} \<union> {X0}"
+    by auto (metis sym_scan.exhaust)
+  show "finite (UNIV :: 'a sym_scan set)"
     by (simp add: * full_SetCompr_eq)
 qed
 
 locale dpda_scan = dpda M for M :: "('q :: finite, 'a :: finite, 's :: finite) pda" 
 begin
 
-definition scan_dpda_final_states :: "'q st_extended set" where
-  "scan_dpda_final_states \<equiv> OST ` final_states M \<union> {F}"
+definition scan_dpda_final_states :: "'q st_scan set" where
+  "scan_dpda_final_states \<equiv> St ` final_states M \<union> {F}"
 
-fun scan_dpda_delta :: "'q st_extended \<Rightarrow> 'a \<Rightarrow> 's sym_extended \<Rightarrow> ('q st_extended \<times> 's sym_extended list) set" where
-  "scan_dpda_delta (OST q) a (OSYM X) = (if \<delta> M q a X = {} \<and> \<delta>\<epsilon> M q X = {} then {(D, [OSYM X])} 
-                                            else (\<lambda>(q, \<alpha>). (OST q, map OSYM \<alpha>)) ` \<delta> M q a X)"
-| "scan_dpda_delta (OST q) _ X0 = {(D, [X0])}"
+fun scan_dpda_delta :: "'q st_scan \<Rightarrow> 'a \<Rightarrow> 's sym_scan \<Rightarrow> ('q st_scan \<times> 's sym_scan list) set" where
+  "scan_dpda_delta (St q) a (Sym X) = (if \<delta> M q a X = {} \<and> \<delta>\<epsilon> M q X = {} then {(D, [Sym X])} 
+                                            else (\<lambda>(q, \<alpha>). (St q, map Sym \<alpha>)) ` \<delta> M q a X)"
+| "scan_dpda_delta (St q) _ X0 = {(D, [X0])}"
 | "scan_dpda_delta D _ X = {(D, [X])}"
 | "scan_dpda_delta _ _ _ = {}"
 
@@ -185,17 +175,21 @@ definition eps_nonfinal :: "'q \<Rightarrow> 's \<Rightarrow> bool" where
 definition eps_final :: "'q \<Rightarrow> 's \<Rightarrow> bool" where
   "eps_final q X \<equiv> (\<forall>i. \<exists>p \<alpha>. (q, [], [X]) \<leadsto>(i) (p, [], \<alpha>)) \<and> (\<exists>i p \<alpha>. (q, [], [X]) \<leadsto>(i) (p, [], \<alpha>) \<and> p \<in> final_states M)"
 
-fun scan_dpda_delta_eps :: "'q st_extended \<Rightarrow> 's sym_extended \<Rightarrow> ('q st_extended \<times> 's sym_extended list) set" where
-  "scan_dpda_delta_eps Q0' X0 = {(OST (init_state M), [OSYM (init_symbol M), X0])}"
-| "scan_dpda_delta_eps (OST q) (OSYM X) = (if eps_nonfinal q X then {(D, [OSYM X])} else
-                                            if eps_final q X then {(F, [OSYM X])} else
-                                              (\<lambda>(q, \<alpha>). (OST q, map OSYM \<alpha>)) ` \<delta>\<epsilon> M q X)"
+fun scan_dpda_delta_eps :: "'q st_scan \<Rightarrow> 's sym_scan \<Rightarrow> ('q st_scan \<times> 's sym_scan list) set" where
+  "scan_dpda_delta_eps Q0' X0 = {(St (init_state M), [Sym (init_symbol M), X0])}"
+| "scan_dpda_delta_eps (St q) (Sym X) = (if eps_nonfinal q X then {(D, [Sym X])} else
+                                            if eps_final q X then {(F, [Sym X])} else
+                                              (\<lambda>(q, \<alpha>). (St q, map Sym \<alpha>)) ` \<delta>\<epsilon> M q X)"
 | "scan_dpda_delta_eps F X = {(D, [X])}"
 | "scan_dpda_delta_eps _ _ = {}"
 
-definition scan_dpda :: "('q st_extended, 'a, 's sym_extended) pda" where
-  "scan_dpda \<equiv> \<lparr> init_state = Q0', init_symbol = X0, final_states = scan_dpda_final_states, 
-                  delta = scan_dpda_delta, delta_eps = scan_dpda_delta_eps \<rparr>"
+definition scan_dpda :: "('q st_scan, 'a, 's sym_scan) pda" where
+  "scan_dpda =
+  \<lparr> init_state = Q0',
+    init_symbol = X0,
+    final_states = scan_dpda_final_states, 
+    delta = scan_dpda_delta, delta_eps = scan_dpda_delta_eps \<rparr>"
+
 
 subsubsection \<open>Determinism\<close>
 
@@ -217,7 +211,7 @@ next
   proof (induction q a X rule: scan_dpda_delta.induct)
     case (1 q a X)
     then show ?case proof
-      assume a: "scan_dpda_delta (OST q) a (OSYM X) \<noteq> {}"
+      assume a: "scan_dpda_delta (St q) a (Sym X) \<noteq> {}"
       have *: "\<delta>\<epsilon> M q X = {}" proof (rule ccontr)
         assume c: "\<delta>\<epsilon> M q X \<noteq> {}"
         from a c have "\<delta> M q a X \<noteq> {}" by simp
@@ -225,12 +219,12 @@ next
           using \<delta>_nonempty[of q a X] by satx
         with c show False by satx
       qed
-      hence **: "(q, [], [X]) \<leadsto>" by simp 
+      hence **: "(q, [], [X]) \<leadsto>|" by simp 
       from ** have ***: "\<not>eps_final q X"
         by (force simp: eps_final_def)
       from ** have ****: "\<not>eps_nonfinal q X"
         by (force simp: eps_nonfinal_def)
-      from * *** **** show "scan_dpda_delta_eps (OST q) (OSYM X) = {}" by simp
+      from * *** **** show "scan_dpda_delta_eps (St q) (Sym X) = {}" by simp
     qed
   qed simp_all
   then show ?case by (simp add: scan_dpda_def)
@@ -246,40 +240,40 @@ next
   then show ?case by (simp add: scan_dpda_def)
 qed
 
+
 subsubsection \<open>Equivalence\<close>
 
 sublocale scan: dpda scan_dpda
   using dpda_scan_dpda .
 
-text \<open>We abbreviate the definitions of @{const [source] scan_dpda} with sub-index s:\<close>
-notation scan.step\<^sub>1 ("(_ \<leadsto>\<^sub>s _)" [50, 50] 50)
-notation scan.steps ("(_ \<leadsto>\<^sub>s* _)" [50, 50] 50)
-notation scan.nstep\<^sub>1 ("(_ \<leadsto>\<^sub>s)" [50] 50)
+text \<open>We abbreviate the definitions of @{const [source] scan_dpda} with index \<open>s\<close>:\<close>
+notation scan.step\<^sub>1 (infix "\<leadsto>\<^sub>s" 55)
+notation scan.steps (infix "\<leadsto>\<^sub>s*" 55)
                                                            
-abbreviation stack_with_X0 :: "'s list \<Rightarrow> 's sym_extended list" where 
-  "stack_with_X0 \<alpha> \<equiv> map OSYM \<alpha> @ [X0]"
+abbreviation stack_with_X0 :: "'s list \<Rightarrow> 's sym_scan list" where 
+  "stack_with_X0 \<alpha> \<equiv> map Sym \<alpha> @ [X0]"
 
 lemma scan_dpda_first_step:
   assumes "(Q0', w, [X0]) \<leadsto>\<^sub>s (q, u, \<alpha>)"
-  shows "q = OST (init_state M) \<and> u = w \<and> \<alpha> = [OSYM (init_symbol M), X0]"
+  shows "q = St (init_state M) \<and> u = w \<and> \<alpha> = [Sym (init_symbol M), X0]"
   using assms scan.step\<^sub>1_rule by (simp add: scan_dpda_def)
 
-lemma scan_dpda_step_from_OST:
-  assumes "(OST q, w, \<alpha>) \<leadsto>\<^sub>s (p, u, \<gamma>)"
-  shows "(\<exists>p'. p = OST p') \<or> p = F \<or> p = D"
+lemma scan_dpda_step_from_St:
+  assumes "(St q, w, \<alpha>) \<leadsto>\<^sub>s (p, u, \<gamma>)"
+  shows "(\<exists>p'. p = St p') \<or> p = F \<or> p = D"
 proof -
   from assms obtain X where
-  "(\<exists>\<beta>. (p, \<beta>) \<in> scan_dpda_delta_eps (OST q) X) \<or> (\<exists>a \<beta>. (p,\<beta>) \<in> scan_dpda_delta (OST q) a X)" (is "?a \<or> ?b")
+  "(\<exists>\<beta>. (p, \<beta>) \<in> scan_dpda_delta_eps (St q) X) \<or> (\<exists>a \<beta>. (p,\<beta>) \<in> scan_dpda_delta (St q) a X)" (is "?a \<or> ?b")
     using scan.step\<^sub>1_rule_ext scan_dpda_def by fastforce
   then consider (a) ?a | (b) ?b by blast
   thus ?thesis
   proof cases
     case a
-    then show ?thesis by (induction "OST q" X rule: scan_dpda_delta_eps.induct) (auto split: if_splits)
+    then show ?thesis by (induction "St q" X rule: scan_dpda_delta_eps.induct) (auto split: if_splits)
   next
     case b
-    then obtain a where "\<exists>\<beta>. (p, \<beta>) \<in> scan_dpda_delta (OST q) a X" by blast
-    then show ?thesis by (induction "OST q" a X rule: scan_dpda_delta.induct) (auto split: if_splits)
+    then obtain a where "\<exists>\<beta>. (p, \<beta>) \<in> scan_dpda_delta (St q) a X" by blast
+    then show ?thesis by (induction "St q" a X rule: scan_dpda_delta.induct) (auto split: if_splits)
   qed
 qed
 
@@ -290,7 +284,7 @@ lemma scan_dpda_step_from_F:
 
 lemma scan_dpda_step_to_F:
   assumes "(q, w, X#\<alpha>) \<leadsto>\<^sub>s (F, u, \<gamma>)"
-  shows "u = w \<and> (\<exists>q' X'. q = OST q' \<and> X = OSYM X' \<and> eps_final q' X')"
+  shows "u = w \<and> (\<exists>q' X'. q = St q' \<and> X = Sym X' \<and> eps_final q' X')"
 proof -
   from assms have cases: "(\<exists>\<beta>. u = w \<and> \<gamma> = \<beta> @ \<alpha> \<and> (F, \<beta>) \<in> scan_dpda_delta_eps q X) 
                       \<or> (\<exists>a \<beta>. w = a # u \<and> \<gamma> = \<beta> @ \<alpha> \<and> (F, \<beta>) \<in> scan_dpda_delta q a X)" (is "?a \<or> ?b")
@@ -312,93 +306,93 @@ lemma scan_dpda_step_from_D:
   shows "q = D"
 using assms scan.step\<^sub>1_rule_ext[of D w \<alpha> q u \<gamma>] scan_dpda_def by auto
 
-lemma scan_dpda_steps_from_OST:
-  assumes "(OST q, w, \<alpha>) \<leadsto>\<^sub>s* (p, u, \<gamma>)"
-  shows "(\<exists>p'. p = OST p') \<or> p = F \<or> p = D"
-using assms by (induction "(OST q, w, \<alpha>)" "(p, u, \<gamma>)" arbitrary: p u \<gamma> rule: scan.steps_induct2_bw, simp) 
- (use scan_dpda_step_from_OST scan_dpda_step_from_F scan_dpda_step_from_D in blast)
+lemma scan_dpda_steps_from_St:
+  assumes "(St q, w, \<alpha>) \<leadsto>\<^sub>s* (p, u, \<gamma>)"
+  shows "(\<exists>p'. p = St p') \<or> p = F \<or> p = D"
+using assms by (induction "(St q, w, \<alpha>)" "(p, u, \<gamma>)" arbitrary: p u \<gamma> rule: scan.steps_induct2_bw, simp) 
+ (use scan_dpda_step_from_St scan_dpda_step_from_F scan_dpda_step_from_D in blast)
 
-lemma scan_dpda_step_to_OST:
-  assumes "(q, w, \<alpha>) \<leadsto>\<^sub>s (OST p, u, \<gamma>)"
-  shows "q = Q0' \<or> (\<exists>q'. q = OST q')"
-using assms scan_dpda_step_from_F[of w \<alpha> "OST p" u \<gamma>] scan_dpda_step_from_D[of w \<alpha> "OST p" u \<gamma>]
-  by (metis st_extended.exhaust st_extended.simps(5))
+lemma scan_dpda_step_to_St:
+  assumes "(q, w, \<alpha>) \<leadsto>\<^sub>s (St p, u, \<gamma>)"
+  shows "q = Q0' \<or> (\<exists>q'. q = St q')"
+using assms scan_dpda_step_from_F[of w \<alpha> "St p" u \<gamma>] scan_dpda_step_from_D[of w \<alpha> "St p" u \<gamma>]
+  by (metis st_scan.exhaust st_scan.simps(5))
 
 lemma scan_dpda_stack_with_X0:
-  assumes "(OST q, w, stack_with_X0 \<alpha>) \<leadsto>\<^sub>s* (OST p, u, \<gamma>)"
+  assumes "(St q, w, stack_with_X0 \<alpha>) \<leadsto>\<^sub>s* (St p, u, \<gamma>)"
   shows "\<exists>\<gamma>'. \<gamma> = stack_with_X0 \<gamma>'"
-using assms proof (induction "(OST q, w, stack_with_X0 \<alpha>)" "(OST p, u, \<gamma>)" arbitrary: p u \<gamma> rule: scan.steps_induct2_bw)
+using assms proof (induction "(St q, w, stack_with_X0 \<alpha>)" "(St p, u, \<gamma>)" arbitrary: p u \<gamma> rule: scan.steps_induct2_bw)
   case (step r u \<gamma> v \<beta>)
-  from step(1,2) obtain r' where r_OST[simp]: "r = OST r'"
-    using scan_dpda_steps_from_OST[of q w "stack_with_X0 \<alpha>" r u \<gamma>] scan_dpda_step_to_OST[of r u \<gamma> p v \<beta>] by blast
-  from step(3)[OF r_OST] obtain \<gamma>'' where \<gamma>_X0: "\<gamma> = stack_with_X0 \<gamma>''" by blast
+  from step(1,2) obtain r' where r_St[simp]: "r = St r'"
+    using scan_dpda_steps_from_St[of q w "stack_with_X0 \<alpha>" r u \<gamma>] scan_dpda_step_to_St[of r u \<gamma> p v \<beta>] by blast
+  from step(3)[OF r_St] obtain \<gamma>'' where \<gamma>_X0: "\<gamma> = stack_with_X0 \<gamma>''" by blast
   from step(2) obtain X \<gamma>' \<beta>' where \<gamma>_def: "\<gamma> = X#\<gamma>'" and \<beta>_def: "\<beta> = \<beta>' @ \<gamma>'" and
-    cases: "(OST p, \<beta>') \<in> scan_dpda_delta_eps (OST r') X \<or> (\<exists>a. (OST p, \<beta>') \<in> scan_dpda_delta (OST r') a X)" (is "?a \<or> ?b")
-    using scan.step\<^sub>1_rule_ext[of r u \<gamma> "OST p" v \<beta>] scan_dpda_def by auto
+    cases: "(St p, \<beta>') \<in> scan_dpda_delta_eps (St r') X \<or> (\<exists>a. (St p, \<beta>') \<in> scan_dpda_delta (St r') a X)" (is "?a \<or> ?b")
+    using scan.step\<^sub>1_rule_ext[of r u \<gamma> "St p" v \<beta>] scan_dpda_def by auto
   from cases consider (a) ?a | (b) ?b by blast
-  then have X_and_\<beta>'_def: "(\<exists>X'. X = OSYM X') \<and> (\<exists>\<beta>''. \<beta>' = map OSYM \<beta>'')"
+  then have X_and_\<beta>'_def: "(\<exists>X'. X = Sym X') \<and> (\<exists>\<beta>''. \<beta>' = map Sym \<beta>'')"
   proof cases
     case a
-    then show ?thesis by (induction "OST r'" X rule: scan_dpda_delta_eps.induct) (auto split: if_splits)
+    then show ?thesis by (induction "St r'" X rule: scan_dpda_delta_eps.induct) (auto split: if_splits)
   next
     case b
-    then obtain a where "(OST p, \<beta>') \<in> scan_dpda_delta (OST r') a X" by blast
-    then show ?thesis by (induction "OST r'" a X rule: scan_dpda_delta.induct) (auto split: if_splits)
+    then obtain a where "(St p, \<beta>') \<in> scan_dpda_delta (St r') a X" by blast
+    then show ?thesis by (induction "St r'" a X rule: scan_dpda_delta.induct) (auto split: if_splits)
   qed
   from X_and_\<beta>'_def[THEN conjunct1] \<gamma>_X0 \<gamma>_def have "\<exists>\<gamma>'''. \<gamma>' = stack_with_X0 \<gamma>'''"
-    by (metis hd_append list.sel(1,3) map_tl sym_extended.distinct(1) tl_append_if)
+    by (metis hd_append list.sel(1,3) map_tl sym_scan.distinct(1) tl_append_if)
   with X_and_\<beta>'_def[THEN conjunct2] \<beta>_def show ?case
     by (metis append.assoc map_append)
 qed blast
 
 lemma scan_dpda_trans:
-  assumes "(OST q, map OSYM \<alpha>) \<in> \<delta> scan_dpda (OST p) a (OSYM X)"
+  assumes "(St q, map Sym \<alpha>) \<in> \<delta> scan_dpda (St p) a (Sym X)"
   shows "(q, \<alpha>) \<in> \<delta> M p a X"
-using assms by (auto simp: scan_dpda_def inj_map_eq_map[OF inj_OSYM] split: if_splits)
+using assms by (auto simp: scan_dpda_def inj_map_eq_map[OF inj_Sym] split: if_splits)
 
 lemma scan_dpda_eps:
-  assumes "(OST q, map OSYM \<alpha>) \<in> \<delta>\<epsilon> scan_dpda (OST p) (OSYM X)"
+  assumes "(St q, map Sym \<alpha>) \<in> \<delta>\<epsilon> scan_dpda (St p) (Sym X)"
   shows "(q, \<alpha>) \<in> \<delta>\<epsilon> M p X"
-using assms by (auto simp: scan_dpda_def inj_map_eq_map[OF inj_OSYM] split: if_splits)
+using assms by (auto simp: scan_dpda_def inj_map_eq_map[OF inj_Sym] split: if_splits)
 
 lemma scan_dpda_step: 
-  assumes "(OST q, w, map OSYM \<alpha>) \<leadsto>\<^sub>s (OST p, u, map OSYM \<gamma>)"
+  assumes "(St q, w, map Sym \<alpha>) \<leadsto>\<^sub>s (St p, u, map Sym \<gamma>)"
   shows "(q, w, \<alpha>) \<leadsto> (p, u, \<gamma>)"
 proof -
-  from assms obtain X \<alpha>' where \<alpha>OSYM_def: "map OSYM \<alpha> = OSYM X # map OSYM \<alpha>'" and rule:
-  "(\<exists>\<beta>. u = w \<and> map OSYM \<gamma> = \<beta> @ map OSYM \<alpha>' \<and> (OST p, \<beta>) \<in> \<delta>\<epsilon> scan_dpda (OST q) (OSYM X)) \<or>
-         (\<exists>a \<beta>. w = a # u \<and> map OSYM \<gamma> = \<beta> @ map OSYM \<alpha>' \<and> (OST p, \<beta>) \<in> \<delta> scan_dpda (OST q) a (OSYM X))"
-    using scan.step\<^sub>1_rule_ext[of "OST q" w "map OSYM \<alpha>" "OST p" u "map OSYM \<gamma>"] by auto
-  from \<alpha>OSYM_def have \<alpha>_def: "\<alpha> = X#\<alpha>'"
-    using inj_map_eq_map[OF inj_OSYM] by auto
-  from rule have "(\<exists>\<beta>. u = w \<and> map OSYM \<gamma> = map OSYM \<beta> @ map OSYM \<alpha>' \<and> (OST p, map OSYM \<beta>) \<in> \<delta>\<epsilon> scan_dpda (OST q) (OSYM X)) \<or>
-         (\<exists>a \<beta>. w = a # u \<and> map OSYM \<gamma> = map OSYM \<beta> @ map OSYM \<alpha>' \<and> (OST p, map OSYM \<beta>) \<in> \<delta> scan_dpda (OST q) a (OSYM X))"
-    using append_eq_map_conv[where ?f = OSYM] by metis
+  from assms obtain X \<alpha>' where \<alpha>Sym_def: "map Sym \<alpha> = Sym X # map Sym \<alpha>'" and rule:
+  "(\<exists>\<beta>. u = w \<and> map Sym \<gamma> = \<beta> @ map Sym \<alpha>' \<and> (St p, \<beta>) \<in> \<delta>\<epsilon> scan_dpda (St q) (Sym X)) \<or>
+         (\<exists>a \<beta>. w = a # u \<and> map Sym \<gamma> = \<beta> @ map Sym \<alpha>' \<and> (St p, \<beta>) \<in> \<delta> scan_dpda (St q) a (Sym X))"
+    using scan.step\<^sub>1_rule_ext[of "St q" w "map Sym \<alpha>" "St p" u "map Sym \<gamma>"] by auto
+  from \<alpha>Sym_def have \<alpha>_def: "\<alpha> = X#\<alpha>'"
+    using inj_map_eq_map[OF inj_Sym] by auto
+  from rule have "(\<exists>\<beta>. u = w \<and> map Sym \<gamma> = map Sym \<beta> @ map Sym \<alpha>' \<and> (St p, map Sym \<beta>) \<in> \<delta>\<epsilon> scan_dpda (St q) (Sym X)) \<or>
+         (\<exists>a \<beta>. w = a # u \<and> map Sym \<gamma> = map Sym \<beta> @ map Sym \<alpha>' \<and> (St p, map Sym \<beta>) \<in> \<delta> scan_dpda (St q) a (Sym X))"
+    using append_eq_map_conv[where ?f = Sym] by metis
   then have "(\<exists>\<beta>. u = w \<and> \<gamma> = \<beta>@\<alpha>' \<and> (p, \<beta>) \<in> \<delta>\<epsilon> M q X) \<or> (\<exists>a \<beta>. w = a#u \<and> \<gamma> = \<beta>@\<alpha>' \<and> (p, \<beta>) \<in> \<delta> M q a X)"
-    using scan_dpda_trans scan_dpda_eps by (metis inj_OSYM inj_map_eq_map map_append)
+    using scan_dpda_trans scan_dpda_eps by (metis inj_Sym inj_map_eq_map map_append)
   with \<alpha>_def show ?thesis
     using step\<^sub>1_rule by simp
 qed  
 
 lemma scan_dpda_stepX0:
-  assumes "(OST q, w, stack_with_X0 \<alpha>) \<leadsto>\<^sub>s (OST p, u, stack_with_X0 \<gamma>)"
+  assumes "(St q, w, stack_with_X0 \<alpha>) \<leadsto>\<^sub>s (St p, u, stack_with_X0 \<gamma>)"
   shows "(q, w, \<alpha>) \<leadsto> (p, u, \<gamma>)"
 proof -
   from assms obtain X \<alpha>' where \<alpha>_def: "stack_with_X0 \<alpha> = X#\<alpha>'" and
-    cases: "(\<exists>\<beta>. (OST p, \<beta>) \<in> scan_dpda_delta_eps (OST q) X) \<or> (\<exists>a \<beta>. (OST p, \<beta>) \<in> scan_dpda_delta (OST q) a X)" (is "?a \<or> ?b")
-    using scan.step\<^sub>1_rule_ext[of "OST q" w "stack_with_X0 \<alpha>" "OST p" u "stack_with_X0 \<gamma>"] scan_dpda_def by force
+    cases: "(\<exists>\<beta>. (St p, \<beta>) \<in> scan_dpda_delta_eps (St q) X) \<or> (\<exists>a \<beta>. (St p, \<beta>) \<in> scan_dpda_delta (St q) a X)" (is "?a \<or> ?b")
+    using scan.step\<^sub>1_rule_ext[of "St q" w "stack_with_X0 \<alpha>" "St p" u "stack_with_X0 \<gamma>"] scan_dpda_def by force
   from cases consider (a) ?a | (b) ?b by blast
-  then have "\<exists>X'. X = OSYM X'"
+  then have "\<exists>X'. X = Sym X'"
   proof cases
     case a
-    then show ?thesis by (induction "OST q" X rule: scan_dpda_delta_eps.induct) auto
+    then show ?thesis by (induction "St q" X rule: scan_dpda_delta_eps.induct) auto
   next
     case b
-    then obtain a where "\<exists>\<beta>. (OST p, \<beta>) \<in> scan_dpda_delta (OST q) a X" by blast
-    then show ?thesis by (induction "OST q" a X rule: scan_dpda_delta.induct) auto
+    then obtain a where "\<exists>\<beta>. (St p, \<beta>) \<in> scan_dpda_delta (St q) a X" by blast
+    then show ?thesis by (induction "St q" a X rule: scan_dpda_delta.induct) auto
   qed
-  with \<alpha>_def have "map OSYM \<alpha> \<noteq> []" by auto
-  then have "(OST q, w, map OSYM \<alpha>) \<leadsto>\<^sub>s (OST p, u, map OSYM \<gamma>)"
+  with \<alpha>_def have "map Sym \<alpha> \<noteq> []" by auto
+  then have "(St q, w, map Sym \<alpha>) \<leadsto>\<^sub>s (St p, u, map Sym \<gamma>)"
     using scan.step\<^sub>1_stack_drop[OF assms] by simp
   then show ?thesis
     using scan_dpda_step by presburger
@@ -406,16 +400,16 @@ qed
 
 text \<open>The original automaton can mimic the steps of the automaton @{const [source] scan_dpda} in the old states:\<close>
 lemma scan_dpda_stepsX0:
-  assumes "(OST q, w, stack_with_X0 \<alpha>) \<leadsto>\<^sub>s* (OST p, u, stack_with_X0 \<gamma>)"
+  assumes "(St q, w, stack_with_X0 \<alpha>) \<leadsto>\<^sub>s* (St p, u, stack_with_X0 \<gamma>)"
   shows "(q, w, \<alpha>) \<leadsto>* (p, u, \<gamma>)"
-using assms proof (induction "(OST q, w, stack_with_X0 \<alpha>)" "(OST p, u, stack_with_X0 \<gamma>)" arbitrary: p u \<gamma> rule: scan.steps_induct2_bw)
+using assms proof (induction "(St q, w, stack_with_X0 \<alpha>)" "(St p, u, stack_with_X0 \<gamma>)" arbitrary: p u \<gamma> rule: scan.steps_induct2_bw)
   case base
   then show ?case
-    by (simp add: inj_OSYM steps_refl)
+    by (simp add: inj_Sym steps_refl)
 next
   case (step r u \<beta> v)
-  obtain r' where r_def: "r = OST r'"
-    using scan_dpda_steps_from_OST[OF step(1)] scan_dpda_step_to_OST[OF step(2)] by blast
+  obtain r' where r_def: "r = St r'"
+    using scan_dpda_steps_from_St[OF step(1)] scan_dpda_step_to_St[OF step(2)] by blast
   obtain \<beta>' where \<beta>_def: "\<beta> = stack_with_X0 \<beta>'"
     using scan_dpda_stack_with_X0[OF step(1)[simplified r_def]] by blast
   from step(3)[OF r_def \<beta>_def] have *: "(q, w, \<alpha>) \<leadsto>* (r', u, \<beta>')" .
@@ -457,8 +451,8 @@ qed
 text \<open>The automaton @{const [source] scan_dpda} can either mimic the steps of the original automaton or detect a cycle:\<close>
 lemma scan_dpda_steps:
   assumes "(q, w, \<alpha>) \<leadsto>* (p, u, \<gamma>)"
-  shows "(OST q, w, map OSYM \<alpha>) \<leadsto>\<^sub>s* (OST p, u, map OSYM \<gamma>) \<or>     
-            (\<exists>r X \<beta>. (OST q, w, map OSYM \<alpha>) \<leadsto>\<^sub>s* (OST r, u, OSYM X # map OSYM \<beta>) \<and> (r, [], X#\<beta>) \<leadsto>* (p, [], \<gamma>) \<and> (\<forall>i. \<exists>s \<Delta>. (r, [], [X]) \<leadsto>(i) (s, [], \<Delta>)))"
+  shows "(St q, w, map Sym \<alpha>) \<leadsto>\<^sub>s* (St p, u, map Sym \<gamma>) \<or>     
+            (\<exists>r X \<beta>. (St q, w, map Sym \<alpha>) \<leadsto>\<^sub>s* (St r, u, Sym X # map Sym \<beta>) \<and> (r, [], X#\<beta>) \<leadsto>* (p, [], \<gamma>) \<and> (\<forall>i. \<exists>s \<Delta>. (r, [], [X]) \<leadsto>(i) (s, [], \<Delta>)))"
 using assms proof (induction "(q, w, \<alpha>)" "(p, u, \<gamma>)" arbitrary: p u \<gamma> rule: steps_induct2_bw)
   case base
   then show ?case
@@ -473,8 +467,8 @@ next
   proof cases
     case a    
     then obtain \<zeta> where v_def: "u = v" and \<beta>_def: "\<beta> = \<zeta> @ \<gamma>'" and elem: "(r, \<zeta>) \<in> \<delta>\<epsilon> M p X" by blast 
-    from step(3) consider (a1) "(OST q, w, map OSYM \<alpha>) \<leadsto>\<^sub>s* (OST p, u, map OSYM \<gamma>)" |  
-                          (a2) "\<exists>r X \<beta>. (OST q, w, map OSYM \<alpha>) \<leadsto>\<^sub>s* (OST r, u, OSYM X # map OSYM \<beta>) \<and> (r, [], X # \<beta>) \<leadsto>* (p, [], \<gamma>) \<and> (\<forall>i. \<exists>s \<Delta>. (r, [], [X]) \<leadsto>(i) (s, [], \<Delta>))" by blast
+    from step(3) consider (a1) "(St q, w, map Sym \<alpha>) \<leadsto>\<^sub>s* (St p, u, map Sym \<gamma>)" |  
+                          (a2) "\<exists>r X \<beta>. (St q, w, map Sym \<alpha>) \<leadsto>\<^sub>s* (St r, u, Sym X # map Sym \<beta>) \<and> (r, [], X # \<beta>) \<leadsto>* (p, [], \<gamma>) \<and> (\<forall>i. \<exists>s \<Delta>. (r, [], [X]) \<leadsto>(i) (s, [], \<Delta>))" by blast
     then show ?thesis
     proof cases    
       case a1   
@@ -482,7 +476,7 @@ next
       then show ?thesis
       proof cases
         case a11     
-        from a1[unfolded v_def \<gamma>_def] have *: "(OST q, w, map OSYM \<alpha>) \<leadsto>\<^sub>s* (OST p, v, OSYM X # map OSYM \<gamma>')" by simp 
+        from a1[unfolded v_def \<gamma>_def] have *: "(St q, w, map Sym \<alpha>) \<leadsto>\<^sub>s* (St p, v, Sym X # map Sym \<gamma>')" by simp 
         from elem \<beta>_def have **: "(p, [], X # \<gamma>') \<leadsto>* (r, [], \<beta>)"
           using step\<^sub>1_rule[of p "[]" X \<gamma>' r "[]" \<beta>] step\<^sub>1_steps by blast 
         from * ** a11 show ?thesis by blast  
@@ -490,16 +484,16 @@ next
         case a12                                                                  
         then have "\<not>eps_nonfinal p X \<and> \<not>eps_final p X"
           by (auto simp: eps_nonfinal_def eps_final_def)
-        with elem have "(OST r, map OSYM \<zeta>) \<in> \<delta>\<epsilon> scan_dpda (OST p) (OSYM X)"
+        with elem have "(St r, map Sym \<zeta>) \<in> \<delta>\<epsilon> scan_dpda (St p) (Sym X)"
           by (auto simp: scan_dpda_def)
-        with v_def \<gamma>_def \<beta>_def have *: "(OST p, u, map OSYM \<gamma>) \<leadsto>\<^sub>s (OST r, v, map OSYM \<beta>)"
-          using scan.step\<^sub>1_rule[of "OST p" u "OSYM X" "map OSYM \<gamma>'" "OST r" u "map OSYM \<zeta> @ map OSYM \<gamma>'"] by simp
+        with v_def \<gamma>_def \<beta>_def have *: "(St p, u, map Sym \<gamma>) \<leadsto>\<^sub>s (St r, v, map Sym \<beta>)"
+          using scan.step\<^sub>1_rule[of "St p" u "Sym X" "map Sym \<gamma>'" "St r" u "map Sym \<zeta> @ map Sym \<gamma>'"] by simp
         show ?thesis
           using scan.steps_trans[OF a1 scan.step\<^sub>1_steps[OF *]] by satx  
       qed               
     next                                               
       case a2         
-      then obtain s Y \<mu> where *: "(OST q, w, map OSYM \<alpha>) \<leadsto>\<^sub>s* (OST s, u, OSYM Y # map OSYM \<mu>)" and spath: "(s, [], Y # \<mu>) \<leadsto>* (p, [], \<gamma>)"
+      then obtain s Y \<mu> where *: "(St q, w, map Sym \<alpha>) \<leadsto>\<^sub>s* (St s, u, Sym Y # map Sym \<mu>)" and spath: "(s, [], Y # \<mu>) \<leadsto>* (p, [], \<gamma>)"
                           and **: "\<forall>i. \<exists>t \<Delta>. (s, [], [Y]) \<leadsto>(i) (t, [], \<Delta>)" by blast 
       from elem \<gamma>_def \<beta>_def have ***:"(p, [], \<gamma>) \<leadsto> (r, [], \<beta>)"   
         using step\<^sub>1_rule[of p "[]" X \<gamma>' r "[]" \<beta>] by simp  
@@ -512,9 +506,9 @@ next
     then obtain a \<zeta> where u_def: "u = a#v" and \<beta>_def: "\<beta> = \<zeta> @ \<gamma>'" and elem: "(r, \<zeta>) \<in> \<delta> M p a X" by blast
     from elem have eps_empty: "\<delta>\<epsilon> M p X = {}"               
       using \<delta>_nonempty[of p a X] by blast
-    from step(3) consider (t) "(OST q, w, map OSYM \<alpha>) \<leadsto>\<^sub>s* (OST p, u, map OSYM \<gamma>)" 
-      | (f) "\<exists>r X \<beta>. (OST q, w, map OSYM \<alpha>) \<leadsto>\<^sub>s* (OST r, u, OSYM X # map OSYM \<beta>) \<and> (r, [], X # \<beta>) \<leadsto>* (p, [], \<gamma>) \<and> (\<forall>i. \<exists>s \<Delta>. (r, [], [X]) \<leadsto>(i) (s, [], \<Delta>))" by blast
-    then have *: "(OST q, w, map OSYM \<alpha>) \<leadsto>\<^sub>s* (OST p, u, map OSYM \<gamma>)"         
+    from step(3) consider (t) "(St q, w, map Sym \<alpha>) \<leadsto>\<^sub>s* (St p, u, map Sym \<gamma>)" 
+      | (f) "\<exists>r X \<beta>. (St q, w, map Sym \<alpha>) \<leadsto>\<^sub>s* (St r, u, Sym X # map Sym \<beta>) \<and> (r, [], X # \<beta>) \<leadsto>* (p, [], \<gamma>) \<and> (\<forall>i. \<exists>s \<Delta>. (r, [], [X]) \<leadsto>(i) (s, [], \<Delta>))" by blast
+    then have *: "(St q, w, map Sym \<alpha>) \<leadsto>\<^sub>s* (St p, u, map Sym \<gamma>)"         
     proof cases
       case t
       then show ?thesis .
@@ -525,20 +519,17 @@ next
         using stack_cycle_drop[OF f2 f1] by blast 
       then obtain n where f3: "(s, [], [Y]) \<leadsto>(n) (p, [], X#\<gamma>'')"
         using stepn_steps[of s "[]" "[Y]" p "[]" "X#\<gamma>''"] by presburger 
-      from eps_empty have f4: "(p, [], X#\<gamma>'') \<leadsto>" by simp
-      from f4 have "(s, [], [Y]) \<leadsto>(Suc n)"
-        using stepn_split_last[of n s "[]" "[Y]"] dpda_stepn_det[OF f3] by fastforce
-      with f2 have False
-        using not_None_eq by blast
-      then show ?thesis by simp            
+      from eps_empty have "(p, [], X#\<gamma>'') \<leadsto>|" by simp
+      with f2 f3 max_eps_steps have False by (meson Suc_n_not_le_n)
+      then show ?thesis ..          
     qed     
-    from eps_empty have "(p, [], [X]) \<leadsto>(1)" by auto
+    from eps_empty have "(p, [], [X]) \<leadsto>|" by auto
     then have "\<not>eps_nonfinal p X \<and> \<not>eps_final p X"   
-      unfolding eps_nonfinal_def eps_final_def using not_None_eq by blast
-    with elem have "(OST r, map OSYM \<zeta>) \<in> \<delta> scan_dpda (OST p) a (OSYM X)" 
+      unfolding eps_nonfinal_def eps_final_def using step\<^sub>1_stepn_one by blast
+    with elem have "(St r, map Sym \<zeta>) \<in> \<delta> scan_dpda (St p) a (Sym X)" 
       by (auto simp: scan_dpda_def)
-    with u_def \<gamma>_def \<beta>_def have **: "(OST p, u, map OSYM \<gamma>) \<leadsto>\<^sub>s (OST r, v, map OSYM \<beta>)"
-      using scan.step\<^sub>1_rule[of "OST p" u "OSYM X" "map OSYM \<gamma>'" "OST r" v "map OSYM \<beta>"] by simp  
+    with u_def \<gamma>_def \<beta>_def have **: "(St p, u, map Sym \<gamma>) \<leadsto>\<^sub>s (St r, v, map Sym \<beta>)"
+      using scan.step\<^sub>1_rule[of "St p" u "Sym X" "map Sym \<gamma>'" "St r" v "map Sym \<beta>"] by simp  
     show ?thesis 
       using scan.steps_trans[OF * scan.step\<^sub>1_steps[OF **]] by simp  
   qed                           
@@ -554,17 +545,17 @@ proof
     assume "w \<in> scan.accept_final"
     then obtain q \<gamma> where q_final: "q \<in> scan_dpda_final_states" and scan_path: "(Q0', w, [X0]) \<leadsto>\<^sub>s* (q, [], \<gamma>)"
       unfolding scan.accept_final_def using scan_dpda_def by auto
-    from q_final have cases: "(\<exists>q' \<in> final_states M. q = OST q') \<or> q = F" (is "?a \<or> ?b")
+    from q_final have cases: "(\<exists>q' \<in> final_states M. q = St q') \<or> q = F" (is "?a \<or> ?b")
       unfolding scan_dpda_final_states_def by auto
     then have "\<exists>p u \<alpha>. (Q0', w, [X0]) \<leadsto>\<^sub>s (p, u, \<alpha>) \<and> (p, u, \<alpha>) \<leadsto>\<^sub>s* (q, [], \<gamma>)"
       using scan.steps_not_refl_split_first[OF scan_path] by blast
-    then have p: "(OST (init_state M), w, [OSYM (init_symbol M), X0]) \<leadsto>\<^sub>s* (q, [], \<gamma>)"
+    then have p: "(St (init_state M), w, [Sym (init_symbol M), X0]) \<leadsto>\<^sub>s* (q, [], \<gamma>)"
       using scan_dpda_first_step by blast
     from cases consider (a) ?a | (b) ?b by blast
     then show "w \<in> accept_final"
     proof cases
       case a
-      then obtain q' where q_def: "q = OST q'" and q'_final: "q' \<in> final_states M" by blast
+      then obtain q' where q_def: "q = St q'" and q'_final: "q' \<in> final_states M" by blast
       from p[simplified q_def] obtain \<gamma>' where \<gamma>_def: "\<gamma> = stack_with_X0 \<gamma>'"
         using scan_dpda_stack_with_X0[of "init_state M" w "[init_symbol M]" q' "[]" \<gamma>] by auto
       from p[simplified q_def \<gamma>_def] have "(init_state M, w, [init_symbol M]) \<leadsto>* (q', [], \<gamma>')"
@@ -573,19 +564,19 @@ proof
         unfolding accept_final_def by blast
     next
       case b
-      obtain p u \<alpha> where fss: "(OST (init_state M), w, [OSYM (init_symbol M), X0]) \<leadsto>\<^sub>s* (p, u, \<alpha>)" 
+      obtain p u \<alpha> where fss: "(St (init_state M), w, [Sym (init_symbol M), X0]) \<leadsto>\<^sub>s* (p, u, \<alpha>)" 
                                           and ls: "(p, u, \<alpha>) \<leadsto>\<^sub>s (F, [], \<gamma>)"
         using scan.steps_not_refl_split_last[OF p[simplified b]] by blast
       obtain X \<alpha>' where \<alpha>_def: "\<alpha> = X#\<alpha>'"
         using scan.step\<^sub>1_nonempty_stack[OF ls] by blast
-      obtain p' X' where u_def: "u = []" and p_def: "p = OST p'" and X_def: "X = OSYM X'" and epath: "eps_final p' X'"
+      obtain p' X' where u_def: "u = []" and p_def: "p = St p'" and X_def: "X = Sym X'" and epath: "eps_final p' X'"
         using scan_dpda_step_to_F[OF ls[simplified \<alpha>_def]] by blast
       from fss[simplified p_def] obtain \<alpha>'' where \<alpha>_with_X0: "\<alpha> = stack_with_X0 \<alpha>''"
         using scan_dpda_stack_with_X0[of "init_state M" w "[init_symbol M]" p' u \<alpha>] by auto
       from fss[simplified p_def u_def \<alpha>_with_X0] have *: "(init_state M, w, [init_symbol M]) \<leadsto>* (p', [], \<alpha>'')"
         using scan_dpda_stepsX0[of "init_state M" w "[init_symbol M]" p' "[]" \<alpha>''] by simp
       from \<alpha>_def \<alpha>_with_X0 X_def obtain \<alpha>''' where \<alpha>''_def: "\<alpha>'' = X'#\<alpha>'''"
-        by (metis Nil_is_map_conv append_Cons append_Nil hd_Cons_tl list.map_sel(1) list.sel(1) sym_extended.distinct(1) sym_extended.inject)
+        by (metis Nil_is_map_conv append_Cons append_Nil hd_Cons_tl list.map_sel(1) list.sel(1) sym_scan.distinct(1) sym_scan.inject)
       from epath[unfolded eps_final_def] obtain i r \<beta> where path: "(p', [], [X']) \<leadsto>(i) (r, [], \<beta>)" and r_final: "r \<in> final_states M" by blast
       from path have "(p', [], [X']) \<leadsto>* (r, [], \<beta>)"
         using stepn_steps[of p' "[]" "[X']" r "[]" \<beta>] by auto
@@ -602,25 +593,25 @@ next
     assume "w \<in> accept_final"
     then obtain q \<gamma> where q_final: "q \<in> final_states M" and p: "(init_state M, w, [init_symbol M]) \<leadsto>* (q, [], \<gamma>)" 
       unfolding accept_final_def by blast                                                        
-    have fs: "(Q0', w, [X0]) \<leadsto>\<^sub>s (OST (init_state M), w, [OSYM (init_symbol M), X0])"
+    have fs: "(Q0', w, [X0]) \<leadsto>\<^sub>s (St (init_state M), w, [Sym (init_symbol M), X0])"
       using scan_dpda_def scan.step\<^sub>1_rule by auto
-    from scan_dpda_steps[OF p] consider (a) "(OST (init_state M), w, [OSYM (init_symbol M)]) \<leadsto>\<^sub>s* (OST q, [], map OSYM \<gamma>)"
-      | (b) "\<exists>r X \<beta>. (OST (init_state M), w, [OSYM (init_symbol M)]) \<leadsto>\<^sub>s* (OST r, [], OSYM X # map OSYM \<beta>) \<and>
+    from scan_dpda_steps[OF p] consider (a) "(St (init_state M), w, [Sym (init_symbol M)]) \<leadsto>\<^sub>s* (St q, [], map Sym \<gamma>)"
+      | (b) "\<exists>r X \<beta>. (St (init_state M), w, [Sym (init_symbol M)]) \<leadsto>\<^sub>s* (St r, [], Sym X # map Sym \<beta>) \<and>
                                 (r, [], X # \<beta>) \<leadsto>* (q, [], \<gamma>) \<and> (\<forall>i. \<exists>s \<Delta>. (r, [], [X]) \<leadsto>(i) (s, [], \<Delta>))" by auto
     then show "w \<in> scan.accept_final"
     proof cases
       case a
-      have "(OST (init_state M), w, [OSYM (init_symbol M), X0]) \<leadsto>\<^sub>s* (OST q, [], stack_with_X0 \<gamma>)"
+      have "(St (init_state M), w, [Sym (init_symbol M), X0]) \<leadsto>\<^sub>s* (St q, [], stack_with_X0 \<gamma>)"
         using scan.steps_stack_app[OF a] by simp
-      then have "(Q0', w, [X0]) \<leadsto>\<^sub>s* (OST q, [], stack_with_X0 \<gamma>)"
-        using scan.step\<^sub>1_steps[OF fs] scan.steps_trans[of Q0' w "[X0]" "OST (init_state M)" w "[OSYM (init_symbol M), X0]" "OST q" "[]" "stack_with_X0 \<gamma>"] by simp 
+      then have "(Q0', w, [X0]) \<leadsto>\<^sub>s* (St q, [], stack_with_X0 \<gamma>)"
+        using scan.step\<^sub>1_steps[OF fs] scan.steps_trans[of Q0' w "[X0]" "St (init_state M)" w "[Sym (init_symbol M), X0]" "St q" "[]" "stack_with_X0 \<gamma>"] by simp 
       with q_final show ?thesis
         unfolding scan.accept_final_def using scan_dpda_def scan_dpda_final_states_def by auto
     next
       case b
-      then obtain r X \<beta> where pscan: "(OST (init_state M), w, [OSYM (init_symbol M)]) \<leadsto>\<^sub>s* (OST r, [], OSYM X # map OSYM \<beta>)" and
+      then obtain r X \<beta> where pscan: "(St (init_state M), w, [Sym (init_symbol M)]) \<leadsto>\<^sub>s* (St r, [], Sym X # map Sym \<beta>)" and
         pr: "(r, [], X # \<beta>) \<leadsto>* (q, [], \<gamma>)" and cycle: "\<forall>i. \<exists>s \<Delta>. (r, [], [X]) \<leadsto>(i) (s, [], \<Delta>)" by blast
-      have *: "(OST (init_state M), w, [OSYM (init_symbol M), X0]) \<leadsto>\<^sub>s* (OST r, [], stack_with_X0 (X # \<beta>))"
+      have *: "(St (init_state M), w, [Sym (init_symbol M), X0]) \<leadsto>\<^sub>s* (St r, [], stack_with_X0 (X # \<beta>))"
         using scan.steps_stack_app[OF pscan] by simp
       have r_final: "\<exists>\<gamma>'. (r, [], [X]) \<leadsto>* (q, [], \<gamma>')"
         using stack_cycle_drop[OF cycle pr] by auto
@@ -628,10 +619,10 @@ next
         unfolding eps_nonfinal_def using stepn_steps[of r "[]" "[X]" q "[]"] dpda_stepn_det[of _ r "[]" "[X]" q "[]"] by blast
       from cycle r_final q_final have e2: "eps_final r X"
         unfolding eps_final_def using stepn_steps[of r "[]" "[X]" q "[]"] by blast
-      from e1 e2 have "(OST r, [], OSYM X # map OSYM \<beta>) \<leadsto>\<^sub>s (F, [], OSYM X # map OSYM \<beta>)"
-        using scan_dpda_def scan.step\<^sub>1_rule[of "OST r" "[]" "OSYM X" "map OSYM \<beta>" F "[]" "OSYM X # map OSYM \<beta>"] by simp
-      then have **: "(OST r, [], stack_with_X0 (X#\<beta>)) \<leadsto>\<^sub>s (F, [], stack_with_X0 (X#\<beta>))"
-        using scan.steps_stack_app[of "OST r" "[]" "OSYM X # map OSYM \<beta>" F "[]" "OSYM X # map OSYM \<beta>"] by simp
+      from e1 e2 have "(St r, [], Sym X # map Sym \<beta>) \<leadsto>\<^sub>s (F, [], Sym X # map Sym \<beta>)"
+        using scan_dpda_def scan.step\<^sub>1_rule[of "St r" "[]" "Sym X" "map Sym \<beta>" F "[]" "Sym X # map Sym \<beta>"] by simp
+      then have **: "(St r, [], stack_with_X0 (X#\<beta>)) \<leadsto>\<^sub>s (F, [], stack_with_X0 (X#\<beta>))"
+        using scan.steps_stack_app[of "St r" "[]" "Sym X # map Sym \<beta>" F "[]" "Sym X # map Sym \<beta>"] by simp
       from fs * ** have "(Q0', w, [X0]) \<leadsto>\<^sub>s* (F, [], stack_with_X0 (X # \<beta>))"
         using scan.step\<^sub>1_steps scan.steps_trans by metis
       then show ?thesis
@@ -639,6 +630,7 @@ next
     qed
   qed                                               
 qed
+
 
 subsubsection \<open>Scan Property\<close>
 
@@ -659,12 +651,12 @@ qed
 definition eps_inf :: "'q \<Rightarrow> 's \<Rightarrow> bool" where
   "eps_inf q X \<equiv> \<forall>i. \<exists>p \<alpha>. (q, [], [X]) \<leadsto>(i) (p, [], \<alpha>)"
 
-definition eps_infl :: "'q \<Rightarrow> 's list \<Rightarrow> bool" where
-  "eps_infl q \<alpha> \<equiv> \<forall>i. \<exists>p \<gamma>. (q, [], \<alpha>) \<leadsto>(i) (p, [], \<gamma>)"
+definition eps_infs :: "'q \<Rightarrow> 's list \<Rightarrow> bool" where
+  "eps_infs q \<alpha> \<equiv> \<forall>i. \<exists>p \<gamma>. (q, [], \<alpha>) \<leadsto>(i) (p, [], \<gamma>)"
 
 text \<open>If a pair of a state and a stack symbol does not allow infinite epsilon steps, then the stack symbol will be consumed:\<close>
 lemma inf_consumes_sym:
-  assumes "eps_infl q (X#\<alpha>)"
+  assumes "eps_infs q (X#\<alpha>)"
       and "\<not>eps_inf q X"
     shows "\<exists>p. (q, [], X#\<alpha>) \<leadsto>* (p, [], \<alpha>)"
 proof (rule ccontr)
@@ -677,7 +669,7 @@ proof (rule ccontr)
   next
     case (Suc i)
     then obtain p \<gamma> where p: "(q, [], X # \<alpha>) \<leadsto>(i) (p, [], \<gamma> @ \<alpha>)" and \<gamma>_def: "\<gamma> \<noteq> []" and p1: "(q, [], [X]) \<leadsto>(i) (p, [], \<gamma>)" by blast
-    from assms(1)[unfolded eps_infl_def] obtain r \<beta> where *: "(q, [], X#\<alpha>) \<leadsto>(Suc i) (r, [], \<beta>)" by blast
+    from assms(1)[unfolded eps_infs_def] obtain r \<beta> where *: "(q, [], X#\<alpha>) \<leadsto>(Suc i) (r, [], \<beta>)" by blast
     then have st: "(p, [], \<gamma>@\<alpha>) \<leadsto> (r, [], \<beta>)"
       using stepn_split_last[of i q "[]" "X#\<alpha>" r "[]" \<beta>] dpda_stepn_det[OF p] by auto
     from \<gamma>_def obtain Y \<gamma>' where \<gamma>_def2: "\<gamma> = Y#\<gamma>'"
@@ -698,13 +690,13 @@ proof (rule ccontr)
 qed
 
 lemma some_pair_inf:
-  assumes "eps_infl q \<alpha>"
+  assumes "eps_infs q \<alpha>"
       and "\<And>p X \<gamma>. (q, [], \<alpha>) \<leadsto>* (p, [], X#\<gamma>) \<longrightarrow> \<not>eps_inf p X"
     shows False
 using assms proof (induction \<alpha> arbitrary: q)
   case Nil
   then show ?case
-    by (force simp: eps_infl_def)
+    by (force simp: eps_infs_def)
 next
   case (Cons X \<alpha>)
   from Cons(3)[of q X \<alpha>] have e: "\<not>eps_inf q X"
@@ -713,9 +705,9 @@ next
     using inf_consumes_sym[OF Cons(2) e] by blast
   then obtain i where p1: "(q, [], X#\<alpha>) \<leadsto>(i) (p, [], \<alpha>)"
     using stepn_steps[of q "[]" "X#\<alpha>" p "[]" \<alpha>] by blast
-  have *: "eps_infl p \<alpha>" unfolding eps_infl_def proof
+  have *: "eps_infs p \<alpha>" unfolding eps_infs_def proof
     fix j
-    from Cons(2)[unfolded eps_infl_def] obtain r \<beta> where p2: "(q, [], X#\<alpha>) \<leadsto>(i + j) (r, [], \<beta>)" by blast
+    from Cons(2)[unfolded eps_infs_def] obtain r \<beta> where p2: "(q, [], X#\<alpha>) \<leadsto>(i + j) (r, [], \<beta>)" by blast
     have "(p, [], \<alpha>) \<leadsto>(j) (r, [], \<beta>)"
       using split_path[OF p2, of i] dpda_stepn_det[OF p1] by auto
     then show "\<exists>r \<beta>. (p, [], \<alpha>) \<leadsto>(j) (r, [], \<beta>)" by blast
@@ -728,31 +720,31 @@ qed
 text \<open>If a configuration allows infinite epsilon steps, it will eventually reach a pair of a 
       state and a stack symbol that allows infinite epsilon steps:\<close>
 lemma inf_reaches:
-  assumes "eps_infl q \<alpha>"
+  assumes "eps_infs q \<alpha>"
   shows "\<exists>p X \<gamma>. (q, [], \<alpha>) \<leadsto>* (p, [], X#\<gamma>) \<and> eps_inf p X"
 using assms some_pair_inf by blast
 
 lemma eps_inf_to_D:
   assumes "eps_inf q X"
-  shows "(OST q, w, OSYM X # \<alpha>) \<leadsto>\<^sub>s* (D, [], OSYM X # \<alpha>)"
+  shows "(St q, w, Sym X # \<alpha>) \<leadsto>\<^sub>s* (D, [], Sym X # \<alpha>)"
 proof -
   from assms consider (a) "eps_nonfinal q X" | (b) "\<not>eps_nonfinal q X \<and> eps_final q X"
     unfolding eps_inf_def eps_nonfinal_def eps_final_def by blast
   then show ?thesis proof cases
     case a
-    then have "(D, [OSYM X]) \<in> scan_dpda_delta_eps (OST q) (OSYM X)" by simp
-    then have st: "(OST q, w, OSYM X # \<alpha>) \<leadsto>\<^sub>s (D, w, OSYM X # \<alpha>)"
-      using scan.step\<^sub>1_rule[of "OST q" w "OSYM X" \<alpha> D w "OSYM X # \<alpha>"] by (simp add: scan_dpda_def)
+    then have "(D, [Sym X]) \<in> scan_dpda_delta_eps (St q) (Sym X)" by simp
+    then have st: "(St q, w, Sym X # \<alpha>) \<leadsto>\<^sub>s (D, w, Sym X # \<alpha>)"
+      using scan.step\<^sub>1_rule[of "St q" w "Sym X" \<alpha> D w "Sym X # \<alpha>"] by (simp add: scan_dpda_def)
     show ?thesis
       using scan.steps_trans[OF scan.step\<^sub>1_steps[OF st] D_consumes] .
   next
     case b
-    then have "(F, [OSYM X]) \<in> scan_dpda_delta_eps (OST q) (OSYM X)" by simp
-    then have st1: "(OST q, w, OSYM X # \<alpha>) \<leadsto>\<^sub>s (F, w, OSYM X # \<alpha>)"
-      using scan.step\<^sub>1_rule[of "OST q" w "OSYM X" \<alpha> F w "OSYM X # \<alpha>"] by (simp add: scan_dpda_def)
-    have "(D, [OSYM X]) \<in> scan_dpda_delta_eps F (OSYM X)" by simp
-    then have st2: "(F, w, OSYM X # \<alpha>) \<leadsto>\<^sub>s (D, w, OSYM X # \<alpha>)"
-      using scan.step\<^sub>1_rule[of F w  "OSYM X" \<alpha> D w "OSYM X # \<alpha>"] by (simp add: scan_dpda_def)
+    then have "(F, [Sym X]) \<in> scan_dpda_delta_eps (St q) (Sym X)" by simp
+    then have st1: "(St q, w, Sym X # \<alpha>) \<leadsto>\<^sub>s (F, w, Sym X # \<alpha>)"
+      using scan.step\<^sub>1_rule[of "St q" w "Sym X" \<alpha> F w "Sym X # \<alpha>"] by (simp add: scan_dpda_def)
+    have "(D, [Sym X]) \<in> scan_dpda_delta_eps F (Sym X)" by simp
+    then have st2: "(F, w, Sym X # \<alpha>) \<leadsto>\<^sub>s (D, w, Sym X # \<alpha>)"
+      using scan.step\<^sub>1_rule[of F w  "Sym X" \<alpha> D w "Sym X # \<alpha>"] by (simp add: scan_dpda_def)
     show ?thesis
       using scan.steps_trans[OF scan.step\<^sub>1_steps[OF st1] scan.steps_trans[OF scan.step\<^sub>1_steps[OF st2] D_consumes]] .
   qed
@@ -761,35 +753,35 @@ qed
 lemma scan_dpda_eps_inf:
   assumes "(q, w, \<alpha>) \<leadsto>* (p, w, X#\<gamma>)"
       and "eps_inf p X"
-    shows "\<exists>Y \<beta>. (OST q, w, map OSYM \<alpha>) \<leadsto>\<^sub>s* (D, [], OSYM Y # \<beta>)"
+    shows "\<exists>Y \<beta>. (St q, w, map Sym \<alpha>) \<leadsto>\<^sub>s* (D, [], Sym Y # \<beta>)"
 proof -
-  consider (a) "(OST q, w, map OSYM \<alpha>) \<leadsto>\<^sub>s* (OST p, w, OSYM X # map OSYM \<gamma>)" |
-           (b) "\<exists>r Y \<beta>. (OST q, w, map OSYM \<alpha>) \<leadsto>\<^sub>s* (OST r, w, OSYM Y # map OSYM \<beta>) \<and> (\<forall>i. \<exists>s \<zeta>. (r, [], [Y]) \<leadsto>(i) (s, [], \<zeta>))"
+  consider (a) "(St q, w, map Sym \<alpha>) \<leadsto>\<^sub>s* (St p, w, Sym X # map Sym \<gamma>)" |
+           (b) "\<exists>r Y \<beta>. (St q, w, map Sym \<alpha>) \<leadsto>\<^sub>s* (St r, w, Sym Y # map Sym \<beta>) \<and> (\<forall>i. \<exists>s \<zeta>. (r, [], [Y]) \<leadsto>(i) (s, [], \<zeta>))"
     using scan_dpda_steps[OF assms(1)] by auto
   then show ?thesis proof cases
     case a
-    have *: "(OST p, w, OSYM X # map OSYM \<gamma>) \<leadsto>\<^sub>s* (D, [], OSYM X # map OSYM \<gamma>)"
+    have *: "(St p, w, Sym X # map Sym \<gamma>) \<leadsto>\<^sub>s* (D, [], Sym X # map Sym \<gamma>)"
       using eps_inf_to_D[OF assms(2)] by simp
     show ?thesis
       using scan.steps_trans[OF a *] by blast
   next
     case b
-    then obtain r Y \<beta> where p: "(OST q, w, map OSYM \<alpha>) \<leadsto>\<^sub>s* (OST r, w, OSYM Y # map OSYM \<beta>)" and r_inf: "\<forall>i. \<exists>s \<zeta>. (r, [], [Y]) \<leadsto>(i) (s, [], \<zeta>)" by blast
+    then obtain r Y \<beta> where p: "(St q, w, map Sym \<alpha>) \<leadsto>\<^sub>s* (St r, w, Sym Y # map Sym \<beta>)" and r_inf: "\<forall>i. \<exists>s \<zeta>. (r, [], [Y]) \<leadsto>(i) (s, [], \<zeta>)" by blast
     from r_inf have r_eps_inf: "eps_inf r Y"
       by (simp add: eps_inf_def)
-    have *: "(OST r, w, OSYM Y # map OSYM \<beta>) \<leadsto>\<^sub>s* (D, [], OSYM Y # map OSYM \<beta>)"
+    have *: "(St r, w, Sym Y # map Sym \<beta>) \<leadsto>\<^sub>s* (D, [], Sym Y # map Sym \<beta>)"
       using eps_inf_to_D[OF r_eps_inf] by simp
     show ?thesis
       using scan.steps_trans[OF p *] by blast
   qed
 qed
 
-lemma scan_dpda_neps_infl:
-  assumes "\<not>eps_infl q \<alpha>"
-  shows "\<exists>p \<gamma>. (OST q, w, map OSYM \<alpha>) \<leadsto>\<^sub>s* (OST p, w, map OSYM \<gamma>) \<and> (\<forall>X \<gamma>'. \<gamma> = X#\<gamma>' \<longrightarrow> \<delta>\<epsilon> M p X = {})"
+lemma scan_dpda_neps_infs:
+  assumes "\<not>eps_infs q \<alpha>"
+  shows "\<exists>p \<gamma>. (St q, w, map Sym \<alpha>) \<leadsto>\<^sub>s* (St p, w, map Sym \<gamma>) \<and> (\<forall>X \<gamma>'. \<gamma> = X#\<gamma>' \<longrightarrow> \<delta>\<epsilon> M p X = {})"
 proof -
-  from assms[unfolded eps_infl_def] obtain i where "\<forall>p \<gamma>. \<not>(q, [], \<alpha>) \<leadsto>(i) (p, [], \<gamma>)" by blast
-  then have "\<exists>j p \<gamma>. j < i \<and> (q, [], \<alpha>) \<leadsto>(j) (p, [], \<gamma>) \<and> (p, [], \<gamma>) \<leadsto>" proof (induction i)
+  from assms[unfolded eps_infs_def] obtain i where "\<forall>p \<gamma>. \<not>(q, [], \<alpha>) \<leadsto>(i) (p, [], \<gamma>)" by blast
+  then have "\<exists>j p \<gamma>. j < i \<and> (q, [], \<alpha>) \<leadsto>(j) (p, [], \<gamma>) \<and> (p, [], \<gamma>) \<leadsto>|" proof (induction i)
     case 0
     then show ?case
       by (auto simp: steps_refl)
@@ -803,27 +795,27 @@ proof -
     next
       case b
       then obtain p \<gamma> where *: "(q, [], \<alpha>) \<leadsto>(i) (p, [], \<gamma>)" by blast
-      with Suc(2) have **: "(p, [], \<gamma>) \<leadsto>"
+      with Suc(2) have **: "(p, [], \<gamma>) \<leadsto>|"
         using decreasing_word step\<^sub>1_steps by fastforce
       from * ** show ?thesis by blast
     qed
   qed
-  then obtain j p \<gamma> where "j < i" and p: "(q, [], \<alpha>) \<leadsto>(j) (p, [], \<gamma>)" and nst: "(p, [], \<gamma>) \<leadsto>" by blast
+  then obtain j p \<gamma> where "j < i" and p: "(q, [], \<alpha>) \<leadsto>(j) (p, [], \<gamma>)" and nst: "(p, [], \<gamma>) \<leadsto>|" by blast
   from p have p1: "(q, [], \<alpha>) \<leadsto>* (p, [], \<gamma>)"
     using stepn_steps[of q "[]" \<alpha> p "[]" \<gamma>] by auto
-  consider (a) "(OST q, [], map OSYM \<alpha>) \<leadsto>\<^sub>s* (OST p, [], map OSYM \<gamma>)" |
-           (b) "\<exists>r X \<beta>. (OST q, [], map OSYM \<alpha>) \<leadsto>\<^sub>s* (OST r, [], OSYM X # map OSYM \<beta>) \<and> (\<forall>i. \<exists>s \<Delta>. (r, [], [X]) \<leadsto>(i) (s, [], \<Delta>))"
+  consider (a) "(St q, [], map Sym \<alpha>) \<leadsto>\<^sub>s* (St p, [], map Sym \<gamma>)" |
+           (b) "\<exists>r X \<beta>. (St q, [], map Sym \<alpha>) \<leadsto>\<^sub>s* (St r, [], Sym X # map Sym \<beta>) \<and> (\<forall>i. \<exists>s \<Delta>. (r, [], [X]) \<leadsto>(i) (s, [], \<Delta>))"
     using scan_dpda_steps[OF p1] by blast
   then show ?thesis proof cases
     case a
-    then have *: "(OST q, w, map OSYM \<alpha>) \<leadsto>\<^sub>s* (OST p, w, map OSYM \<gamma>)"
-      using scan.steps_word_app[of "OST q" "[]" "map OSYM \<alpha>" "OST p" "[]" "map OSYM \<gamma>" w] by simp
+    then have *: "(St q, w, map Sym \<alpha>) \<leadsto>\<^sub>s* (St p, w, map Sym \<gamma>)"
+      using scan.steps_word_app[of "St q" "[]" "map Sym \<alpha>" "St p" "[]" "map Sym \<gamma>" w] by simp
     from nst have **: "\<forall>X \<gamma>'. \<gamma> = X # \<gamma>' \<longrightarrow> \<delta>\<epsilon> M p X = {}" by auto
     from * ** show ?thesis by blast
   next
     case b
-    then obtain r X \<beta> where p2: "(OST q, [], map OSYM \<alpha>) \<leadsto>\<^sub>s* (OST r, [], OSYM X # map OSYM \<beta>)" and cycle: "\<forall>i. \<exists>s \<Delta>. (r, [], [X]) \<leadsto>(i) (s, [], \<Delta>)" by blast
-    from p2 have p3: "(OST q, [], stack_with_X0 \<alpha>) \<leadsto>\<^sub>s* (OST r, [], stack_with_X0 (X#\<beta>))"
+    then obtain r X \<beta> where p2: "(St q, [], map Sym \<alpha>) \<leadsto>\<^sub>s* (St r, [], Sym X # map Sym \<beta>)" and cycle: "\<forall>i. \<exists>s \<Delta>. (r, [], [X]) \<leadsto>(i) (s, [], \<Delta>)" by blast
+    from p2 have p3: "(St q, [], stack_with_X0 \<alpha>) \<leadsto>\<^sub>s* (St r, [], stack_with_X0 (X#\<beta>))"
       using scan.steps_stack_app[where ?\<beta> = "[X0]"] by fastforce
     have "(q, [], \<alpha>) \<leadsto>* (r, [], X#\<beta>)"
       using scan_dpda_stepsX0[OF p3] .
@@ -850,30 +842,30 @@ proof -
       qed
     qed
     with assms show ?thesis
-      by (simp add: eps_infl_def)
+      by (simp add: eps_infs_def)
   qed
 qed
 
-lemma scan_dpda_scans_OST:
-"\<exists>p X \<gamma>. (OST q, w, stack_with_X0 \<alpha>) \<leadsto>\<^sub>s* (p, [], X#\<gamma>) \<and> \<delta> scan_dpda p a X \<noteq> {}"
+lemma scan_dpda_scans_St:
+"\<exists>p X \<gamma>. (St q, w, stack_with_X0 \<alpha>) \<leadsto>\<^sub>s* (p, [], X#\<gamma>) \<and> \<delta> scan_dpda p a X \<noteq> {}"
 proof (induction w arbitrary: q \<alpha>)
   case Nil
-  then show ?case proof (cases "eps_infl q \<alpha>")
+  then show ?case proof (cases "eps_infs q \<alpha>")
     case True
     obtain p X \<gamma> where p: "(q, [], \<alpha>) \<leadsto>* (p, [], X#\<gamma>)" and eps_p: "eps_inf p X"
       using inf_reaches[OF True] by blast
-    obtain Y \<beta> where "(OST q, [], map OSYM \<alpha>) \<leadsto>\<^sub>s* (D, [], OSYM Y # \<beta>)"
+    obtain Y \<beta> where "(St q, [], map Sym \<alpha>) \<leadsto>\<^sub>s* (D, [], Sym Y # \<beta>)"
       using scan_dpda_eps_inf[OF p eps_p] by blast
-    then have *: "(OST q, [], stack_with_X0 \<alpha>) \<leadsto>\<^sub>s* (D, [], OSYM Y # \<beta> @ [X0])"
+    then have *: "(St q, [], stack_with_X0 \<alpha>) \<leadsto>\<^sub>s* (D, [], Sym Y # \<beta> @ [X0])"
       using scan.steps_stack_app[where ?\<beta> = "[X0]"] by fastforce
-    have **: "\<delta> scan_dpda D a (OSYM Y) \<noteq> {}"
+    have **: "\<delta> scan_dpda D a (Sym Y) \<noteq> {}"
       by (simp add: scan_dpda_def)
     from * ** show ?thesis by blast
   next
     case False
-    obtain p \<gamma> where p: "(OST q, [], map OSYM \<alpha>) \<leadsto>\<^sub>s* (OST p, [], map OSYM \<gamma>)" and \<gamma>_nempty: "(\<forall>X \<gamma>'. \<gamma> = X#\<gamma>' \<longrightarrow> \<delta>\<epsilon> M p X = {})"
-      using scan_dpda_neps_infl[OF False] by blast
-    from p have p1: "(OST q, [], stack_with_X0 \<alpha>) \<leadsto>\<^sub>s* (OST p, [], stack_with_X0 \<gamma>)"
+    obtain p \<gamma> where p: "(St q, [], map Sym \<alpha>) \<leadsto>\<^sub>s* (St p, [], map Sym \<gamma>)" and \<gamma>_nempty: "(\<forall>X \<gamma>'. \<gamma> = X#\<gamma>' \<longrightarrow> \<delta>\<epsilon> M p X = {})"
+      using scan_dpda_neps_infs[OF False] by blast
+    from p have p1: "(St q, [], stack_with_X0 \<alpha>) \<leadsto>\<^sub>s* (St p, [], stack_with_X0 \<gamma>)"
       using scan.steps_stack_app[where ?\<beta> = "[X0]"] by simp
     show ?thesis proof (cases \<gamma>)
       case Nil
@@ -882,38 +874,38 @@ proof (induction w arbitrary: q \<alpha>)
     next
       case (Cons X \<gamma>')
       with \<gamma>_nempty have "\<delta>\<epsilon> M p X = {}" by simp
-      then have "\<delta> scan_dpda (OST p) a (OSYM X) \<noteq> {}"
+      then have "\<delta> scan_dpda (St p) a (Sym X) \<noteq> {}"
         by (simp add: scan_dpda_def)
       with p1 Cons show ?thesis by auto
     qed
   qed
 next
   case IH: (Cons b w)
-  show ?case proof (cases "eps_infl q \<alpha>")
+  show ?case proof (cases "eps_infs q \<alpha>")
     case True
     obtain p X \<gamma> where p: "(q, [], \<alpha>) \<leadsto>* (p, [], X#\<gamma>)" and eps_p: "eps_inf p X"
       using inf_reaches[OF True] by blast
     from p have p1: "(q, b#w, \<alpha>) \<leadsto>* (p, b#w, X#\<gamma>)"
       using steps_word_app[of q "[]" \<alpha> p "[]" "X#\<gamma>" "b#w"] by simp
-    obtain Y \<beta> where "(OST q, b # w, map OSYM \<alpha>) \<leadsto>\<^sub>s* (D, [], OSYM Y # \<beta>)"
+    obtain Y \<beta> where "(St q, b # w, map Sym \<alpha>) \<leadsto>\<^sub>s* (D, [], Sym Y # \<beta>)"
       using scan_dpda_eps_inf[OF p1 eps_p] by blast
-    then have *: "(OST q, b # w, stack_with_X0 \<alpha>) \<leadsto>\<^sub>s* (D, [], OSYM Y # \<beta> @ [X0])"
+    then have *: "(St q, b # w, stack_with_X0 \<alpha>) \<leadsto>\<^sub>s* (D, [], Sym Y # \<beta> @ [X0])"
       using scan.steps_stack_app[where ?\<beta> = "[X0]"] by fastforce
-    have **: "\<delta> scan_dpda D a (OSYM Y) \<noteq> {}"
+    have **: "\<delta> scan_dpda D a (Sym Y) \<noteq> {}"
       by (simp add: scan_dpda_def)
     from * ** show ?thesis by blast
   next
     case False
-    obtain p \<gamma> where p: "(OST q, b#w, map OSYM \<alpha>) \<leadsto>\<^sub>s* (OST p, b#w, map OSYM \<gamma>)" and \<gamma>_nempty: "(\<forall>X \<gamma>'. \<gamma> = X#\<gamma>' \<longrightarrow> \<delta>\<epsilon> M p X = {})"
-      using scan_dpda_neps_infl[OF False] by blast
-    from p have p1: "(OST q, b#w, stack_with_X0 \<alpha>) \<leadsto>\<^sub>s* (OST p, b#w, stack_with_X0 \<gamma>)"
+    obtain p \<gamma> where p: "(St q, b#w, map Sym \<alpha>) \<leadsto>\<^sub>s* (St p, b#w, map Sym \<gamma>)" and \<gamma>_nempty: "(\<forall>X \<gamma>'. \<gamma> = X#\<gamma>' \<longrightarrow> \<delta>\<epsilon> M p X = {})"
+      using scan_dpda_neps_infs[OF False] by blast
+    from p have p1: "(St q, b#w, stack_with_X0 \<alpha>) \<leadsto>\<^sub>s* (St p, b#w, stack_with_X0 \<gamma>)"
       using scan.steps_stack_app[where ?\<beta> = "[X0]"] by simp
     show ?thesis proof (cases \<gamma>)
       case Nil
-      have "(D, [X0]) \<in> scan_dpda_delta (OST p) b X0" by simp
-      with Nil have st: "(OST p, b#w, stack_with_X0 \<gamma>) \<leadsto>\<^sub>s (D, w, [X0])"
-        using scan.step\<^sub>1_rule[of "OST p" "b#w" X0 "[]" D w "[X0]"] by (simp add: scan_dpda_def)
-      have *: "(OST q, b#w, stack_with_X0 \<alpha>) \<leadsto>\<^sub>s* (D, [], [X0])"
+      have "(D, [X0]) \<in> scan_dpda_delta (St p) b X0" by simp
+      with Nil have st: "(St p, b#w, stack_with_X0 \<gamma>) \<leadsto>\<^sub>s (D, w, [X0])"
+        using scan.step\<^sub>1_rule[of "St p" "b#w" X0 "[]" D w "[X0]"] by (simp add: scan_dpda_def)
+      have *: "(St q, b#w, stack_with_X0 \<alpha>) \<leadsto>\<^sub>s* (D, [], [X0])"
         using scan.steps_trans[OF p1 scan.steps_trans[OF scan.step\<^sub>1_steps[OF st] D_consumes]] .
       have **: "\<delta> scan_dpda D a X0 \<noteq> {}"
         by (simp add: scan_dpda_def)
@@ -921,23 +913,23 @@ next
     next
       case (Cons X \<gamma>')
       with \<gamma>_nempty have "\<delta>\<epsilon> M p X = {}" by simp
-      then consider (a) "(D, [OSYM X]) \<in> scan_dpda_delta (OST p) b (OSYM X)" | (b) "\<exists>r \<beta>. (OST r, map OSYM \<beta>) \<in> scan_dpda_delta (OST p) b (OSYM X)"
+      then consider (a) "(D, [Sym X]) \<in> scan_dpda_delta (St p) b (Sym X)" | (b) "\<exists>r \<beta>. (St r, map Sym \<beta>) \<in> scan_dpda_delta (St p) b (Sym X)"
         by (cases "\<delta> M p b X = {}") fastforce+
       then show ?thesis proof cases
         case a
-        with Cons have st: "(OST p, b#w, stack_with_X0 \<gamma>) \<leadsto>\<^sub>s (D, w, stack_with_X0 \<gamma>)"
-          using scan.step\<^sub>1_rule[of "OST p" "b#w" "OSYM X" "stack_with_X0 \<gamma>'" D w "stack_with_X0 \<gamma>"] by (simp add: scan_dpda_def)
-        from Cons have *: "(OST q, b#w, stack_with_X0 \<alpha>) \<leadsto>\<^sub>s* (D, [], stack_with_X0 \<gamma>)"
-          using scan.steps_trans[OF p1 scan.steps_trans[OF scan.step\<^sub>1_steps[OF st]]] D_consumes[of w "OSYM X" "stack_with_X0 \<gamma>'"] by simp
-        have **: "\<delta> scan_dpda D a (OSYM X) \<noteq> {}"
+        with Cons have st: "(St p, b#w, stack_with_X0 \<gamma>) \<leadsto>\<^sub>s (D, w, stack_with_X0 \<gamma>)"
+          using scan.step\<^sub>1_rule[of "St p" "b#w" "Sym X" "stack_with_X0 \<gamma>'" D w "stack_with_X0 \<gamma>"] by (simp add: scan_dpda_def)
+        from Cons have *: "(St q, b#w, stack_with_X0 \<alpha>) \<leadsto>\<^sub>s* (D, [], stack_with_X0 \<gamma>)"
+          using scan.steps_trans[OF p1 scan.steps_trans[OF scan.step\<^sub>1_steps[OF st]]] D_consumes[of w "Sym X" "stack_with_X0 \<gamma>'"] by simp
+        have **: "\<delta> scan_dpda D a (Sym X) \<noteq> {}"
           by (simp add: scan_dpda_def)
         from * ** Cons show ?thesis by auto
       next
         case b
-        then obtain r \<beta> where "(OST r, map OSYM \<beta>) \<in> scan_dpda_delta (OST p) b (OSYM X)" by blast
-        with Cons have st: "(OST p, b#w, stack_with_X0 \<gamma>) \<leadsto>\<^sub>s (OST r, w, stack_with_X0 (\<beta>@\<gamma>'))"
-          using scan.step\<^sub>1_rule[of "OST p" "b#w" "OSYM X" "stack_with_X0 \<gamma>'" "OST r" w "stack_with_X0 (\<beta>@\<gamma>')"] by (simp add: scan_dpda_def)
-        from IH have *: "\<exists>p X \<gamma>. (OST r, w, stack_with_X0 (\<beta>@\<gamma>')) \<leadsto>\<^sub>s* (p, [], X # \<gamma>) \<and> \<delta> scan_dpda p a X \<noteq> {}" by presburger
+        then obtain r \<beta> where "(St r, map Sym \<beta>) \<in> scan_dpda_delta (St p) b (Sym X)" by blast
+        with Cons have st: "(St p, b#w, stack_with_X0 \<gamma>) \<leadsto>\<^sub>s (St r, w, stack_with_X0 (\<beta>@\<gamma>'))"
+          using scan.step\<^sub>1_rule[of "St p" "b#w" "Sym X" "stack_with_X0 \<gamma>'" "St r" w "stack_with_X0 (\<beta>@\<gamma>')"] by (simp add: scan_dpda_def)
+        from IH have *: "\<exists>p X \<gamma>. (St r, w, stack_with_X0 (\<beta>@\<gamma>')) \<leadsto>\<^sub>s* (p, [], X # \<gamma>) \<and> \<delta> scan_dpda p a X \<noteq> {}" by presburger
         from * show ?thesis
           using scan.steps_trans[OF scan.steps_trans[OF p1 scan.step\<^sub>1_steps[OF st]]] by blast
       qed
@@ -950,17 +942,18 @@ text \<open>For every input word, the automaton @{const [source] scan_dpda} scan
 lemma scan_dpda_scans:
 "\<exists>q X \<alpha>. (init_state scan_dpda, w, [init_symbol scan_dpda]) \<leadsto>\<^sub>s* (q, [], X#\<alpha>) \<and> \<delta> scan_dpda q a X \<noteq> {}"
 proof -
-  have "(OST (init_state M), stack_with_X0 [init_symbol M]) \<in> scan_dpda_delta_eps Q0' X0" by simp
-  then have *: "(init_state scan_dpda, w, [init_symbol scan_dpda]) \<leadsto>\<^sub>s (OST (init_state M), w, stack_with_X0 [init_symbol M])"
-    using scan.step\<^sub>1_rule[of Q0' w X0 "[]" "OST (init_state M)" w "stack_with_X0 [init_symbol M]"] by (simp add: scan_dpda_def)
-  obtain p X \<gamma> where **: "(OST (init_state M), w, stack_with_X0 [init_symbol M]) \<leadsto>\<^sub>s* (p, [], X#\<gamma>)" and d: "\<delta> scan_dpda p a X \<noteq> {}"
-    using scan_dpda_scans_OST[of "init_state M" w "[init_symbol M]"] by blast
+  have "(St (init_state M), stack_with_X0 [init_symbol M]) \<in> scan_dpda_delta_eps Q0' X0" by simp
+  then have *: "(init_state scan_dpda, w, [init_symbol scan_dpda]) \<leadsto>\<^sub>s (St (init_state M), w, stack_with_X0 [init_symbol M])"
+    using scan.step\<^sub>1_rule[of Q0' w X0 "[]" "St (init_state M)" w "stack_with_X0 [init_symbol M]"] by (simp add: scan_dpda_def)
+  obtain p X \<gamma> where **: "(St (init_state M), w, stack_with_X0 [init_symbol M]) \<leadsto>\<^sub>s* (p, [], X#\<gamma>)" and d: "\<delta> scan_dpda p a X \<noteq> {}"
+    using scan_dpda_scans_St[of "init_state M" w "[init_symbol M]"] by blast
   have "(init_state scan_dpda, w, [init_symbol scan_dpda]) \<leadsto>\<^sub>s* (p, [], X#\<gamma>)"
     using scan.steps_trans[OF scan.step\<^sub>1_steps[OF *] **] .
   with d show ?thesis by blast
 qed
 
 end
+
 
 subsection \<open>Complement Construction\<close>
 
@@ -969,17 +962,18 @@ text \<open>After ensuring that the automaton scans its entire input word, we ar
       state has been visited since the last true step using a second component for states. If no final state has been 
       visited, the complement automaton enters a final state of its own just before the next true step.\<close>
 
+
 subsubsection \<open>Definition\<close>
 
 text \<open>An S1-state indicates that a final state has been visited since the last true step, whereas an S2-state indicates 
       that no final state has been visited since the last true step. S3-states are the final states of the complement automaton:\<close>
-datatype 'q st_num = S1 'q | S2 'q | S3 'q
+datatype 'q s123 = S1 'q | S2 'q | S3 'q
 
-instance st_num :: (finite) finite
+instance s123 :: (finite) finite
 proof
   have *: "UNIV = {t. \<exists>q. t = S1 q} \<union> {t. \<exists>q. t = S2 q} \<union> {t. \<exists>q. t = S3 q}"
-    by auto (metis st_num.exhaust)
-  show "finite (UNIV :: 'a st_num set)"
+    by auto (metis s123.exhaust)
+  show "finite (UNIV :: 'a s123 set)"
     by (simp add: * full_SetCompr_eq)
 qed
 
@@ -994,26 +988,30 @@ locale complement_dpda = dpda M for M :: "('q :: finite, 'a :: finite, 's :: fin
   assumes M_path: "\<exists>q X \<alpha>. (init_state M, w, [init_symbol M]) \<leadsto>* (q, [], X#\<alpha>) \<and> \<delta> M q a X \<noteq> {}"
 begin
 
-definition comp_dpda_init_state :: "'q st_num" where
+definition comp_dpda_init_state :: "'q s123" where
   "comp_dpda_init_state \<equiv> if init_state M \<in> final_states M then S1 (init_state M) else S2 (init_state M)"
 
-definition comp_dpda_final_states :: "'q st_num set" where
+definition comp_dpda_final_states :: "'q s123 set" where
   "comp_dpda_final_states \<equiv> range S3"
 
-fun comp_dpda_delta :: "'q st_num \<Rightarrow> 'a \<Rightarrow> 's \<Rightarrow> ('q st_num \<times> 's list) set" where
+fun comp_dpda_delta :: "'q s123 \<Rightarrow> 'a \<Rightarrow> 's \<Rightarrow> ('q s123 \<times> 's list) set" where
   "comp_dpda_delta (S1 q) a X = (\<lambda>(p, \<alpha>). if p \<in> final_states M then (S1 p, \<alpha>) else (S2 p, \<alpha>)) ` \<delta> M q a X"
 | "comp_dpda_delta (S3 q) a X = (\<lambda>(p, \<alpha>). if p \<in> final_states M then (S1 p, \<alpha>) else (S2 p, \<alpha>)) ` \<delta> M q a X"
 | "comp_dpda_delta _ _ _ = {}"
 
-fun comp_dpda_delta_eps :: "'q st_num \<Rightarrow> 's \<Rightarrow> ('q st_num \<times> 's list) set" where
+fun comp_dpda_delta_eps :: "'q s123 \<Rightarrow> 's \<Rightarrow> ('q s123 \<times> 's list) set" where
   "comp_dpda_delta_eps (S1 q) X = (\<lambda>(p, \<alpha>). (S1 p, \<alpha>)) ` \<delta>\<epsilon> M q X"
 | "comp_dpda_delta_eps (S2 q) X = (\<lambda>(p, \<alpha>). if p \<in> final_states M then (S1 p, \<alpha>) else (S2 p, \<alpha>)) ` \<delta>\<epsilon> M q X 
                                     \<union> (if \<exists>a. \<delta> M q a X \<noteq> {} then {(S3 q, [X])} else {})"
 | "comp_dpda_delta_eps _ _ = {}"
 
-definition comp_dpda :: "('q st_num, 'a, 's) pda" where
-  "comp_dpda \<equiv> \<lparr> init_state = comp_dpda_init_state, init_symbol = init_symbol M, final_states = comp_dpda_final_states,
-                    delta = comp_dpda_delta, delta_eps = comp_dpda_delta_eps \<rparr>"
+definition comp_dpda :: "('q s123, 'a, 's) pda" where
+  "comp_dpda =
+  \<lparr> init_state = comp_dpda_init_state,
+    init_symbol = init_symbol M,
+    final_states = comp_dpda_final_states,
+    delta = comp_dpda_delta, delta_eps = comp_dpda_delta_eps \<rparr>"
+
 
 subsubsection \<open>Determinism\<close>
 
@@ -1094,17 +1092,17 @@ next
     by (simp add: comp_dpda_def)
 qed
 
+
 subsubsection \<open>Complementation\<close>
 
 sublocale comp: dpda comp_dpda
   using dpda_comp_dpda . 
 
-text \<open>We abbreviate the definitions of @{const [source] comp_dpda} with sub-index c:\<close>
-notation comp.step\<^sub>1 ("(_ \<leadsto>\<^sub>c _)" [50, 50] 50)
-notation comp.steps ("(_ \<leadsto>\<^sub>c* _)" [50, 50] 50)
-notation comp.nstep\<^sub>1 ("(_ \<leadsto>\<^sub>c)" [50] 50)
-notation comp.stepsn ("(_ /\<leadsto>\<^sub>c'(_')/ _)" [50, 0, 50] 50)
-notation comp.stepst ("(_ \<leadsto>\<^sub>c+ _)" [50, 50] 50)
+text \<open>We abbreviate the definitions of @{const [source] comp_dpda} with index \<open>c\<close>:\<close>
+notation comp.step\<^sub>1 (infix "\<leadsto>\<^sub>c" 55)
+notation comp.steps (infix "\<leadsto>\<^sub>c*" 55)
+notation comp.stepsn ("(_ /\<leadsto>\<^sub>c'(_')/ _)" [55, 0, 55] 55)
+notation comp.steps1 (infix "\<leadsto>\<^sub>c+" 55)
 
 lemma comp_dpda_step_from_S1:
   assumes "(S1 q, [], \<alpha>) \<leadsto>\<^sub>c (p, [], \<gamma>)"
@@ -1243,9 +1241,9 @@ lemma comp_dpda_final_steps:
       and "p \<in> final_states M"
       and "q = S1 q' \<or> q = S2 q'"
     shows "(q, w, \<alpha>) \<leadsto>\<^sub>c+ (S1 p, u, \<gamma>)"
-using assms proof (induction "(q', w, \<alpha>)" "(p, u, \<gamma>)" arbitrary: q q' w \<alpha> rule: stepst_induct2)
-  case (1 q' w \<alpha>)
-  from 1(1) obtain X \<alpha>' where \<alpha>_def: "\<alpha> = X#\<alpha>'" and cases:
+using assms proof (induction "(q', w, \<alpha>)" "(p, u, \<gamma>)" arbitrary: q q' w \<alpha> rule: steps1_induct)
+  case (base q' w \<alpha>)
+  from base(1) obtain X \<alpha>' where \<alpha>_def: "\<alpha> = X#\<alpha>'" and cases:
       "(\<exists>\<beta>. u = w \<and> \<gamma> = \<beta> @ \<alpha>' \<and> (p, \<beta>) \<in> \<delta>\<epsilon> M q' X) \<or> (\<exists>a \<beta>. w = a # u \<and> \<gamma> = \<beta> @ \<alpha>' \<and> (p, \<beta>) \<in> \<delta> M q' a X)" (is "?a \<or> ?b")
     using step\<^sub>1_rule_ext[of q' w \<alpha> p u \<gamma>] by blast
   from cases consider (a) ?a | (b) ?b by blast
@@ -1253,41 +1251,41 @@ using assms proof (induction "(q', w, \<alpha>)" "(p, u, \<gamma>)" arbitrary: q
   proof cases
     case a
     then obtain \<beta> where *: "u = w" and **: "\<gamma> = \<beta> @ \<alpha>'" and elem: "(p, \<beta>) \<in> \<delta>\<epsilon> M q' X" by blast
-    from 1(2,3) elem have "(S1 p, \<beta>) \<in> comp_dpda_delta_eps q X" by force
+    from base(2,3) elem have "(S1 p, \<beta>) \<in> comp_dpda_delta_eps q X" by force
     with * ** \<alpha>_def have ***: "(q, w, \<alpha>) \<leadsto>\<^sub>c (S1 p, u, \<gamma>)"
       using comp.step\<^sub>1_rule[of q w X \<alpha>' "S1 p" u \<gamma>] by (simp add: comp_dpda_def)
     show ?thesis
-      using comp.stepst_step[OF ***] .
+      using comp.steps1_step[OF ***] .
   next
     case b
     then obtain a \<beta> where *: "w = a # u" and **: "\<gamma> = \<beta> @ \<alpha>'" and elem: "(p, \<beta>) \<in> \<delta> M q' a X" by blast
-    from 1(3) consider (c) "q = S1 q'" | (d) "q = S2 q'" by blast
+    from base(3) consider (c) "q = S1 q'" | (d) "q = S2 q'" by blast
     then show ?thesis
     proof cases
       case c
-      with elem 1(2) have "(S1 p, \<beta>) \<in> comp_dpda_delta q a X" by force
+      with elem base(2) have "(S1 p, \<beta>) \<in> comp_dpda_delta q a X" by force
       with * ** \<alpha>_def have ***: "(q, w, \<alpha>) \<leadsto>\<^sub>c (S1 p, u, \<gamma>)"
         using comp.step\<^sub>1_rule[of q w X \<alpha>' "S1 p" u \<gamma>] by (simp add: comp_dpda_def)
       show ?thesis
-        using comp.stepst_step[OF ***] .
+        using comp.steps1_step[OF ***] .
     next
       case d
       with elem have "(S3 q', [X]) \<in> comp_dpda_delta_eps q X" by auto
       with \<alpha>_def have ***: "(q, w, \<alpha>) \<leadsto>\<^sub>c (S3 q', w, \<alpha>)"
         using comp.step\<^sub>1_rule[of q w X \<alpha>' "S3 q'" w \<alpha>] by (simp add: comp_dpda_def)
-      from elem 1(2) have "(S1 p, \<beta>) \<in> comp_dpda_delta (S3 q') a X" by force
+      from elem base(2) have "(S1 p, \<beta>) \<in> comp_dpda_delta (S3 q') a X" by force
       with * ** \<alpha>_def have ****: "(S3 q', w, \<alpha>) \<leadsto>\<^sub>c (S1 p, u, \<gamma>)"
         using comp.step\<^sub>1_rule[of "S3 q'" w X \<alpha>' "S1 p" u \<gamma>] by (simp add: comp_dpda_def)
       show ?thesis
-        using comp.stepst_trans[OF comp.stepst_step[OF ***] comp.stepst_step[OF ****]] .
+        using comp.steps1_trans[OF comp.steps1_step[OF ***] comp.steps1_step[OF ****]] .
     qed
   qed
 next
-  case (2 q' w \<alpha> r v \<beta>)
-  from 2(1) obtain X \<alpha>' where \<alpha>_def: "\<alpha> = X#\<alpha>'" and cases:
+  case (step q' w \<alpha> r v \<beta>)
+  from step(1) obtain X \<alpha>' where \<alpha>_def: "\<alpha> = X#\<alpha>'" and cases:
       "(\<exists>\<beta>'. v = w \<and> \<beta> = \<beta>' @ \<alpha>' \<and> (r, \<beta>') \<in> \<delta>\<epsilon> M q' X) \<or> (\<exists>a \<beta>'. w = a # v \<and> \<beta> = \<beta>' @ \<alpha>' \<and> (r, \<beta>') \<in> \<delta> M q' a X)" (is "?c \<or> ?d")
     using step\<^sub>1_rule_ext[of q' w \<alpha> r v \<beta>] by blast
-  from 2(5) consider (a) "q = S1 q'" | (b) "q = S2 q'" by blast
+  from step(5) consider (a) "q = S1 q'" | (b) "q = S2 q'" by blast
   then show ?case
   proof cases
     case a
@@ -1299,19 +1297,19 @@ next
       from elem a have "(S1 r, \<zeta>) \<in> comp_dpda_delta_eps q X" by auto
       with * ** \<alpha>_def have ***: "(q, w, \<alpha>) \<leadsto>\<^sub>c (S1 r, v, \<beta>)"
         using comp.step\<^sub>1_rule[of q w X \<alpha>' "S1 r" v \<beta>] by (simp add: comp_dpda_def)
-      from 2(3)[OF 2(4)] have ****: "(S1 r, v, \<beta>) \<leadsto>\<^sub>c+ (S1 p, u, \<gamma>)" by simp
+      from step(3)[OF step(4)] have ****: "(S1 r, v, \<beta>) \<leadsto>\<^sub>c+ (S1 p, u, \<gamma>)" by simp
       show ?thesis
-        using comp.stepst_trans[OF comp.stepst_step[OF ***] ****] .
+        using comp.steps1_trans[OF comp.steps1_step[OF ***] ****] .
     next
       case d
       then obtain a \<zeta> where *: "w = a # v" and **: "\<beta> = \<zeta> @ \<alpha>'" and elem: "(r, \<zeta>) \<in> \<delta> M q' a X" by blast
       from elem a have "(S1 r, \<zeta>) \<in> comp_dpda_delta q a X \<or> (S2 r, \<zeta>) \<in> comp_dpda_delta q a X" by force
       with * ** \<alpha>_def have ***: "(q, w, \<alpha>) \<leadsto>\<^sub>c (S1 r, v, \<beta>) \<or> (q, w, \<alpha>) \<leadsto>\<^sub>c (S2 r, v, \<beta>)"
         using comp.step\<^sub>1_rule[of q w X \<alpha>' _ v \<beta>] by (simp add: comp_dpda_def)
-      from 2(3)[OF 2(4)] have ****: "(S1 r, v, \<beta>) \<leadsto>\<^sub>c+ (S1 p, u, \<gamma>)" by simp 
-      from 2(3)[OF 2(4)] have *****: "(S2 r, v, \<beta>) \<leadsto>\<^sub>c+ (S1 p, u, \<gamma>)" by simp
+      from step(3)[OF step(4)] have ****: "(S1 r, v, \<beta>) \<leadsto>\<^sub>c+ (S1 p, u, \<gamma>)" by simp 
+      from step(3)[OF step(4)] have *****: "(S2 r, v, \<beta>) \<leadsto>\<^sub>c+ (S1 p, u, \<gamma>)" by simp
       from *** **** ***** show ?thesis
-        using comp.stepst_step comp.stepst_trans by blast
+        using comp.steps1_step comp.steps1_trans by blast
     qed
   next
     case b
@@ -1323,10 +1321,10 @@ next
       from elem b have "(S1 r, \<zeta>) \<in> comp_dpda_delta_eps q X \<or> (S2 r, \<zeta>) \<in> comp_dpda_delta_eps q X" by force
       with * ** \<alpha>_def have ***: "(q, w, \<alpha>) \<leadsto>\<^sub>c (S1 r, v, \<beta>) \<or> (q, w, \<alpha>) \<leadsto>\<^sub>c (S2 r, v, \<beta>)"
         using comp.step\<^sub>1_rule[of q w X \<alpha>' _ v \<beta>] by (simp add: comp_dpda_def)
-      from 2(3)[OF 2(4)] have ****: "(S1 r, v, \<beta>) \<leadsto>\<^sub>c+ (S1 p, u, \<gamma>)" by simp 
-      from 2(3)[OF 2(4)] have *****: "(S2 r, v, \<beta>) \<leadsto>\<^sub>c+ (S1 p, u, \<gamma>)" by simp
+      from step(3)[OF step(4)] have ****: "(S1 r, v, \<beta>) \<leadsto>\<^sub>c+ (S1 p, u, \<gamma>)" by simp 
+      from step(3)[OF step(4)] have *****: "(S2 r, v, \<beta>) \<leadsto>\<^sub>c+ (S1 p, u, \<gamma>)" by simp
       from *** **** ***** show ?thesis
-        using comp.stepst_step comp.stepst_trans by blast
+        using comp.steps1_step comp.steps1_trans by blast
     next
       case d
       then obtain a \<zeta> where *: "w = a # v" and **: "\<beta> = \<zeta> @ \<alpha>'" and elem: "(r, \<zeta>) \<in> \<delta> M q' a X" by blast
@@ -1336,10 +1334,10 @@ next
       from elem have "(S1 r, \<zeta>) \<in> comp_dpda_delta (S3 q') a X \<or> (S2 r, \<zeta>) \<in> comp_dpda_delta (S3 q') a X" by force
       with * ** \<alpha>_def have ****: "(S3 q', w, \<alpha>) \<leadsto>\<^sub>c (S1 r, v, \<beta>) \<or> (S3 q', w, \<alpha>) \<leadsto>\<^sub>c (S2 r, v, \<beta>)"
         using comp.step\<^sub>1_rule[of "S3 q'" w X \<alpha>' _ v \<beta>] by (simp add: comp_dpda_def)
-      from 2(3)[OF 2(4)] have *****: "(S1 r, v, \<beta>) \<leadsto>\<^sub>c+ (S1 p, u, \<gamma>)" by simp
-      from 2(3)[OF 2(4)] have ******: "(S2 r, v, \<beta>) \<leadsto>\<^sub>c+ (S1 p, u, \<gamma>)" by simp
+      from step(3)[OF step(4)] have *****: "(S1 r, v, \<beta>) \<leadsto>\<^sub>c+ (S1 p, u, \<gamma>)" by simp
+      from step(3)[OF step(4)] have ******: "(S2 r, v, \<beta>) \<leadsto>\<^sub>c+ (S1 p, u, \<gamma>)" by simp
       from *** **** ***** ****** show ?thesis
-        using comp.stepst_step comp.stepst_trans by metis
+        using comp.steps1_step comp.steps1_trans by metis
     qed
   qed
 qed
@@ -1354,7 +1352,7 @@ proof
   assume r_final: "r \<in> final_states M"
   from assms(1) obtain n where p1: "(S1 q, w, \<alpha>) \<leadsto>\<^sub>c(n) (S3 p, [], \<gamma>)"
     using comp.stepn_steps[of "S1 q" w \<alpha> "S3 p" "[]" \<gamma>] by blast
-  have np: "(S3 p, [], \<gamma>) \<leadsto>\<^sub>c"
+  have np: "comp.no_step\<^sub>1 (S3 p, [], \<gamma>)"
     using comp.step\<^sub>1_rule_ext[of "S3 p" "[]" \<gamma>] by (simp add: comp_dpda_def)
   have "(S1 q, w, \<alpha>) \<leadsto>\<^sub>c* (S1 r, [], \<beta>)"
   proof (cases "(q, w, \<alpha>) = (r, [], \<beta>)")
@@ -1364,11 +1362,11 @@ proof
   next
     case False
     have q1: "(q, w, \<alpha>) \<leadsto>+ (r, [], \<beta>)"
-      using steps_stepst[OF assms(2) False] .
+      using steps_steps1[OF assms(2) False] .
     have q2: "(S1 q, w, \<alpha>) \<leadsto>\<^sub>c+ (S1 r, [], \<beta>)"
       using comp_dpda_final_steps[OF q1 r_final] by simp
     show ?thesis
-      using comp.stepst_steps[OF q2] .
+      using comp.steps1_steps[OF q2] .
   qed
   then obtain m where p2: "(S1 q, w, \<alpha>) \<leadsto>\<^sub>c(m) (S1 r, [], \<beta>)"
     using comp.stepn_steps[of "S1 q" w \<alpha> "S1 r" "[]" \<beta>] by blast 
@@ -1390,10 +1388,10 @@ proof
   assume r_final: "r \<in> final_states M"
   from assms(1) obtain n where p1: "(S2 q, w, \<alpha>) \<leadsto>\<^sub>c(n) (S3 p, [], \<gamma>)"
     using comp.stepn_steps[of "S2 q" w \<alpha> "S3 p" "[]" \<gamma>] by blast
-  have np: "(S3 p, [], \<gamma>) \<leadsto>\<^sub>c"
+  have np: "comp.no_step\<^sub>1 (S3 p, [], \<gamma>)"
     using comp.step\<^sub>1_rule_ext[of "S3 p" "[]" \<gamma>] by (simp add: comp_dpda_def)
   obtain m where p2: "(S2 q, w, \<alpha>) \<leadsto>\<^sub>c(m) (S1 r, [], \<beta>)"
-    using comp.stepst_steps[OF comp_dpda_final_steps[OF assms(2) r_final, of "S2 q", simplified]] comp.stepn_steps[of "S2 q" w \<alpha> "S1 r" "[]" \<beta>] by blast
+    using comp.steps1_steps[OF comp_dpda_final_steps[OF assms(2) r_final, of "S2 q", simplified]] comp.stepn_steps[of "S2 q" w \<alpha> "S1 r" "[]" \<beta>] by blast
   have m_leq_n: "m \<le> n"
     using comp.max_eps_steps[OF p1 np p2] .
   have "(S1 r, [], \<beta>) \<leadsto>\<^sub>c(n - m) (S3 p, [], \<gamma>)"
@@ -1406,7 +1404,7 @@ qed
 
 text \<open>The language of the automaton @{const [source] comp_dpda} is the complement language:\<close>
 lemma lang_comp_dpda:
-"comp.accept_final = - accept_final"
+  "comp.accept_final = - accept_final"
 proof
   show "comp.accept_final \<subseteq> - accept_final"
   proof
@@ -1438,7 +1436,7 @@ proof
         next
           case d
           then have *: "(init_state M, w, [init_symbol M]) \<leadsto>+ (r, [], \<beta>)"
-            using steps_stepst[OF asm] by simp
+            using steps_steps1[OF asm] by simp
           from b p q_def have **: "(S2 (init_state M), w, [init_symbol M]) \<leadsto>\<^sub>c* (S3 q', [], \<gamma>)"
             by (simp add: comp_dpda_def comp_dpda_init_state_def)
           show ?thesis
@@ -1485,16 +1483,17 @@ text \<open>By constructing the two automata one after another, we get the final
       context-free languages are closed under complementation:\<close>
 lemma complement_dpda:
   assumes "dpda (M :: ('q :: finite, 'a :: finite, 's :: finite) pda)"
-  shows "\<exists>(M' :: ('q st_extended st_num, 'a, 's sym_extended) pda). dpda M' \<and> pda.accept_final M' = - pda.accept_final M"
+  shows "\<exists>M' :: ('q st_scan s123, 'a, 's sym_scan) pda.
+    dpda M' \<and> pda.accept_final M' = - pda.accept_final M"
 proof -
-  let ?SM = "dpda_scan.scan_dpda M :: ('q st_extended, 'a, 's sym_extended) pda"
+  let ?SM = "dpda_scan.scan_dpda M :: ('q st_scan, 'a, 's sym_scan) pda"
   have dpda_sm: "dpda ?SM"
     using assms dpda_scan.dpda_scan_dpda dpda_scan_def by blast
   have *: "\<And>a w. \<exists>q X \<alpha>. pda.steps ?SM (init_state ?SM, w, [init_symbol ?SM]) (q, [], X#\<alpha>) \<and> delta ?SM q a X \<noteq> {}"
     using assms dpda_scan.scan_dpda_scans dpda_scan_def by blast
   have L1: "pda.accept_final ?SM = pda.accept_final M"
     using assms dpda_scan.lang_scan_dpda dpda_scan.intro by auto
-  let ?CM = "complement_dpda.comp_dpda ?SM :: ('q st_extended st_num, 'a, 's sym_extended) pda"
+  let ?CM = "complement_dpda.comp_dpda ?SM :: ('q st_scan s123, 'a, 's sym_scan) pda"
   from dpda_sm * have dpda_cm: "dpda ?CM"
     using complement_dpda.dpda_comp_dpda complement_dpda.intro complement_dpda_axioms_def by blast
   from dpda_sm * have L2: "pda.accept_final ?CM = UNIV - pda.accept_final ?SM"
